Remove KOSBTM and rework TM-computable to BSM-computable
- Remove files KOSBTM.v, HaltTM_1_to_HaltKOSBTM.v, HaltKOSBTM_to_HaltBSM.v.
- Add output lemma to HaltTM_1_to_SBTM_HALT.v
- Adapt construction and add output lemma to SBTM_HALT_to_HaltBSM.v
- Rework TM_computable_to_BSM_computable.v to use SBTM instead of KOSBTM

theories/StackMachines/Reductions/TM_computable_to_BSM_computable.v
@@ -1,16 +1,30 @@
 Set Default Goal Selector "!".
 
-Require Import
+Require Import 
   Undecidability.StackMachines.BSM Undecidability.StackMachines.Util.BSM_computable
   Undecidability.TM.TM Undecidability.TM.Util.TM_facts Undecidability.TM.Util.TM_computable.
-From Undecidability.TM Require Import TM Arbitrary_to_Binary mTM_to_TM HaltTM_1_to_HaltKOSBTM HaltKOSBTM_to_HaltBSM.
+From Undecidability.StackMachines Require Import SBTM_HALT_to_HaltBSM.
+From Undecidability.TM Require Import TM Arbitrary_to_Binary mTM_to_TM HaltTM_1_to_SBTM_HALT.
 From Undecidability.Shared.Libs.DLW Require Import vec pos sss subcode.
 From Undecidability Require Import bsm_utils bsm_defs.
 Require Import Undecidability.TM.Code.Code.
 From Undecidability.Shared.Libs.PSL Require FinTypes.
 From Undecidability.TM Require Import Single.EncodeTapes.
+From Undecidability.TM Require Import SBTM.
+From Undecidability.StackMachines Require Import BSM BSM.bsm_defs.
 
-Notation "v @[ t ]" := (Vector.nth v t) (at level 50).
+Create HintDb vec_simpl discriminated.
+
+Hint Rewrite vec_change_eq using easy : vec_simpl.
+Hint Rewrite vec_change_neq using easy : vec_simpl.
+
+Notation "P // s -[ k ]-> t" := (sss_steps (@bsm_sss _) P k s t).
+Notation "P // s ->> t" := (sss_compute (@bsm_sss _) P s t).
+Notation "P // s ~~> t" := (sss_output (@bsm_sss _) P s t).
+
+(*--- Utility ---*)
+
+Notation "v @[ t ]" := (Vector.nth v t).
 Local Hint Rewrite map_app  : list.
 
 Lemma skipn_app' (X : Type) (xs ys : list X) (n : nat) :
@@ -55,22 +69,19 @@ Lemma vector_inv_back {X n} (v : Vector.t X (S n)) E :
   { '(x, v') : X * Vector.t X n | v = Vector.cast (Vector.append v' (x ## vec_nil)) E }.
 Proof.
   destruct E. 
-  destruct (Vector.splitat n v) eqn:E.
+  destruct (Vector.splitat n v) as [t t0] eqn:E.
   eexists (vec_head t0, t).
-  erewrite <- Vector.append_splitat. 1: now rewrite cast_eq_refl.
+  erewrite <- Vector.append_splitat; [now rewrite cast_eq_refl|].
   rewrite E. f_equal. eapply (Vector.caseS' t0). cbn.
-  intros h. eapply Vector.case0. reflexivity.
+  intros ?. now eapply Vector.case0.
 Qed.
 
 Lemma nth_error_vec_list {X n} (v : Vector.t X n) m (H : m < n) x :
   nth_error (vec_list v) m = Some x ->
   vec_pos v (Fin.of_nat_lt H) = x.
 Proof.
-  induction v in m , H |- *; cbn.
-  - lia.
-  - destruct m; cbn.
-    + congruence.
-    + eapply IHv.
+  induction v as [| ??? IHv] in m, H |- *; cbn; [lia|].
+  destruct m; cbn; [congruence | now apply IHv].
 Qed.
 
 Lemma vec_list_cast {X n} (v :Vector.t X n) m (E : n = m) :
@@ -102,56 +113,77 @@ Lemma update_app_right {X} (x : X) l1 l2 i :
   i >= length l1 ->
   update i (l1 ++ l2) x = l1 ++ update (i - length l1) l2 x.
 Proof.
-  induction l1 in i |- *; cbn.
-  - now rewrite Nat.sub_0_r.
-  - intros Hi. destruct i. 1: lia.
-    cbn. rewrite IHl1. 1: reflexivity. lia.
+  induction l1 as [|?? IHl1] in i |- *; cbn; [now rewrite Nat.sub_0_r |].
+  intros Hi. destruct i; [lia|].
+  cbn. rewrite IHl1; [reflexivity| lia].
 Qed.
 
 Lemma update_app_left {X} (x : X) l1 l2 i : 
   i < length l1 ->
   update i (l1 ++ l2) x = update i l1 x ++ l2.
 Proof.
-  induction l1 in i |- *; cbn.
-  - lia. 
-  - intros Hi. destruct i; cbn.
-    + reflexivity.
-    + rewrite IHl1. 1: reflexivity. lia.
+  induction l1 as [|?? IHl1] in i |- *; cbn; [lia|].
+  intros Hi. destruct i; cbn; [reflexivity|].
+  rewrite IHl1; [reflexivity|lia].
 Qed.
 
 Lemma vec_list_vec_change {X n} (v : Vector.t X n) (x : X) (p : pos n) :
   vec_list (vec_change v p x) = update (proj1_sig (Fin.to_nat p)) (vec_list v) x.
 Proof.
-  induction v; cbn.
+  induction v as [|??? IHv]; cbn.
   - inversion p.
-  - eapply (Fin.caseS' p); cbn.
-    + cbn. reflexivity. 
-    + intros. specialize (IHv p0). destruct (Fin.to_nat p0) eqn:E. cbn in *. now f_equal.
+  - eapply (Fin.caseS' p); cbn; [reflexivity|].
+    intros p0. specialize (IHv p0). destruct (Fin.to_nat p0) eqn:E. cbn in *. now f_equal.
 Qed.
 
-Definition complete_encode (Σ : finType) n (t : Vector.t (tape Σ) n) :=
-  (conv_tape [| encode_tape' (Vector.nth (mTM_to_TM.enc_tape [] t) Fin0) |]).
-
-Lemma KOSBTM_complete_simulation n Σ (M : TM Σ n) :
-  {M' : KOSBTM.KOSBTM |
-        (forall q t t', TM.eval M (TM.start M) t q t' -> exists q', KOSBTM.eval M' Fin.F1 (complete_encode t) q' (complete_encode t')) /\
-        (forall t, (exists q' t', KOSBTM.eval M' Fin.F1 (complete_encode t) q' t') -> (exists q' t', TM.eval M (TM.start M) t q' t'))}.
+Lemma vec_change_app_right {X} (n m : nat) v1 v2 p x:
+  vec_change (@vec_app X n m v1 v2) (pos_right n p) x = vec_app v1 (vec_change v2 p x).
 Proof.
-  destruct (TM_sTM_simulation M) as (M1 & Hf1 & Hb1).
-  destruct (binary_simulation M1) as (M2 & Hf2 & Hb2).
-  destruct (KOSBTM_simulation M2) as (M3 & Hf3 & Hb3).
-  exists M3. split.
-  - intros q t t' [q1 [q2 [q3 H] % Hf3] % Hf2] % Hf1. eexists. eapply H.
-  - intros t H % Hb3 % Hb2 % Hb1. exact H.
+  induction v1 as [| ??? IHv1].
+  - rewrite !vec_app_nil. reflexivity.
+  - rewrite !vec_app_cons. cbn. now rewrite IHv1.
 Qed.
 
-Definition bsm_addstracks' n m (P : bsm_instr n) : (bsm_instr (m + n)) :=
-  (fun x => match x with
-  | bsm_pop x c1 c2 => bsm_pop (pos_right m x) c1 c2
-  | bsm_push x b => bsm_push (pos_right m x) b end) P.
+Lemma pos_right_left {n m} p q : @pos_left n m p <> @pos_right n m q.
+Proof.
+  induction n; cbn.
+  - inversion p.
+  - eapply (Fin.caseS' p).
+    + cbn. congruence.
+    + cbn. intros ? ? % pos_nxt_inj. firstorder.
+Qed.
 
-Definition bsm_addstacks n m (P : list (bsm_instr n)) : list (bsm_instr (m + n)):=
-  map (@bsm_addstracks' n m) P.
+Lemma pos_left_right {n m} p q : @pos_right n m q <> @pos_left n m p.
+Proof.
+  induction n; cbn.
+  - inversion p.
+  - eapply (Fin.caseS' p).
+    + cbn. congruence.
+    + cbn. intros ? ? % pos_nxt_inj. firstorder.
+Qed.
+
+Local Hint Immediate pos_left_right pos_right_left : core.
+
+Lemma vec_change_app_left {X} (n m : nat) v1 v2 p x:
+  vec_change (@vec_app X n m v1 v2) (pos_left m p) x = vec_app (vec_change v1 p x) v2.
+Proof.
+  eapply vec_pos_ext. eapply pos_left_right_rect.
+  - intros p0. rewrite !vec_pos_app_left.
+    destruct (pos_eq_dec p p0).
+    + subst. rewrite vec_change_eq; [|reflexivity]. now rewrite vec_change_eq.
+    + rewrite vec_change_neq; [|intros ? % pos_left_inj; congruence].
+      rewrite vec_pos_app_left. rewrite vec_change_neq; auto.
+  - intros p0. rewrite !vec_pos_app_right. rewrite vec_change_neq; auto. now rewrite vec_pos_app_right.
+Qed.
+
+Lemma vec_app_inj {X} (n m : nat) v1 v2 v2' :
+  @vec_app X n m v1 v2 = vec_app v1 v2' -> v2 = v2'.
+Proof.
+  induction v1 as [| ??? IHv1].
+  - now rewrite !vec_app_nil.
+  - rewrite !vec_app_cons. intros H. eapply IHv1.
+    now eapply (f_equal (@vec_tail _ _)) in H.
+Qed.
 
 Lemma vec_pos_spec {k} {X} (p : pos k) (v : Vector.t X k) : vec_pos v p = Vector.nth v p.
 Proof.
@@ -162,57 +194,233 @@ Proof.
     + intros. cbn. eauto.
 Qed.
 
-Lemma vec_change_app_right {X} (n m : nat) v1 v2 p x:
-  vec_change (@vec_app X n m v1 v2) (pos_right n p) x = vec_app v1 (vec_change v2 p x).
+Lemma pos_right_inj {n m} p q :
+  @pos_right n m p = @pos_right n m q -> p = q.
 Proof.
-  induction v1.
-  - rewrite !vec_app_nil. reflexivity.
-  - rewrite !vec_app_cons. cbn. now rewrite IHv1.
+  induction n as [|n IHn] in p, q |- *; cbn in *.
+  - eauto.
+  - intros H. eapply IHn, pos_nxt_inj, H.
+Qed.
+
+Lemma vec_pos_const {k} {X x} (p : pos k) : vec_pos (@Vector.const X x k) p = x.
+Proof.
+  induction p; cbn; eauto.
+Qed.
+
+Lemma vec_map_spec {X Y n} (v : Vector.t X n) (f : X -> Y) :
+  vec_map f v = Vector.map f v.
+Proof.
+  induction v; cbn; congruence.
+Qed.
+
+Lemma pos_left_inj {n m} p q :
+  @pos_left n m p = @pos_left n m q -> p = q.
+Proof.
+  induction p as [| ? ? IHp] in q |- *; cbn in *.
+  - eapply (Fin.caseS' q).
+    + reflexivity.
+    + clear q. cbn. congruence.
+  - eapply (Fin.caseS' q).
+    + cbn. congruence.
+    + clear q. cbn. intros. f_equal. eapply IHp.
+      now eapply pos_nxt_inj.
+Qed.
+
+(* Utility lemmas for BSM instructions*)
+Lemma POP_true_spec m (STACK : Fin.t m) n t j v v' k1 k2 :
+  vec_pos v STACK = true :: v' ->
+  bsm_sss (POP STACK k1 k2) (j, v) (n, t) ->
+  n = j + 1 /\ t = vec_change v STACK v'.
+Proof.
+  intros H H0.
+  inversion H0 as [????? H1|?????? H1 | ?????? H1 | ]; subst; try clear H0; 
+  rewrite H1 in H; [inversion H | inversion H |].
+  injection H. clear H. intros H. subst. split; [lia | reflexivity].
+Qed.
+
+Lemma POP_false_spec m (STACK : Fin.t m) n t j v v' k1 k2 :
+  vec_pos v STACK = false :: v' ->
+  bsm_sss (POP STACK k1 k2) (j, v) (n, t) ->
+  n = k1 /\ t = vec_change v STACK v'.
+Proof.
+  intros H H0.
+  inversion H0 as [????? H1|?????? H1 | ?????? H1 | ]; subst; try clear H0; rewrite H1 in H; [inversion H |  | inversion H].
+  injection H. clear H. intros H. subst. split; [lia | reflexivity].
+Qed.
+
+Lemma POP_empty_spec m (STACK : Fin.t m) n t j v k1 k2 :
+  vec_pos v STACK = [] ->
+  bsm_sss (POP STACK k1 k2) (j, v) (n, t) ->
+  n = k2 /\ v = t.
+Proof.
+  intros H H0.
+  inversion H0 as [????? H1|?????? H1 | ?????? H1 | ]; subst; try clear H0; rewrite H1 in H; [| inversion H | inversion H].
+  now split.
+Qed.
+
+Lemma POP_empty_spec' m (STACK1 STACK2 : Fin.t m) n t j v k1 k2 :
+  vec_pos v STACK1 = [] ->
+  bsm_sss (POP STACK2 k1 k2) (j, v) (n, t) ->
+  vec_pos t STACK1 = [].
+Proof.
+  intros H0 H1.
+  destruct (vec_pos v STACK2) as [| b l] eqn:E.
+  - apply POP_empty_spec in H1; [| apply E].
+    destruct H1 as [H1 ?]. subst. apply H0.
+  - destruct b; [apply POP_true_spec with (v' := l) in H1; [| apply E]| apply POP_false_spec with (v' := l) in H1; [| apply E]].
+    all: destruct H1; subst; rewrite vec_change_neq; [apply H0|];
+    assert (NEQ : STACK2 <> STACK1); [| apply NEQ];
+    unfold "<>"; intros H3; rewrite <- H3 in H0; rewrite E in H0; inversion H0.
+Qed.
+
+Lemma PUSH_spec (STACK : Fin.t 5) n t j v b :
+  bsm_sss (PUSH STACK b) (j, v) (n, t) ->
+  n = j + 1 /\ t = vec_change v STACK (b :: (vec_pos v STACK)).
+Proof.
+  intros H0.
+  inv H0.
+  now split; [lia | reflexivity].
+Qed.
+
+(* Utility function and lemmas for truncation*)
+Fixpoint remove_leading_falses (l : list bool) :=
+  match l with
+  | false :: l' => remove_leading_falses l'
+  | l' => l'
+  end.
+
+Lemma rev_forallb (A : Type) P (l : list A):
+  forallb P (rev l) =  forallb P l.
+Proof. 
+  induction l as [| a l IHl]; [reflexivity|].
+  cbn.
+  rewrite forallb_app, IHl.
+  cbn.
+  now rewrite andb_true_r, andb_comm.
+Qed.
+
+Lemma leading_false_spec v1 : exists n, (exists l, v1 = repeat false n ++ true :: l) \/ v1 = repeat false n.
+Proof.
+  induction v1 as [| a l IHv1]; [exists 0; now right |].
+  destruct IHv1 as [n [IHv1 | IHv1]]; [destruct IHv1 as [l' IHv1]|]; subst.
+  - destruct a; [exists 0 | exists (S n)]; left; eexists _; now reflexivity.
+  - destruct a.
+      + exists 0. left. eexists _. now reflexivity.
+      + exists (S n). right. now reflexivity.
+Qed.
+
+Lemma remove_leading_falses_spec_false_only n :
+  remove_leading_falses (repeat false n) = [].
+Proof.
+  induction n as [| ? IHn]; [reflexivity | apply IHn].
+Qed.
+
+Lemma remove_leading_falses_dist (l l1 :list bool) : 
+  remove_leading_falses (l ++ true :: l1) = remove_leading_falses l ++ true :: l1.
+Proof.
+  induction l as [| a ? IHl]; [reflexivity|].
+  destruct a; [reflexivity| apply IHl].
+Qed.
+
+Lemma remove_leading_falses_spec l n :
+  remove_leading_falses (repeat false n ++ true :: l) = true :: l.
+Proof.
+  now rewrite remove_leading_falses_dist, remove_leading_falses_spec_false_only.
+Qed.
+
+Lemma true_not_repeat_false x x0 :
+  forallb negb (repeat false x ++ true :: x0) = false.
+Proof.
+  rewrite forallb_app.
+  now destruct (forallb negb (repeat false x)).
+Qed.
+
+Lemma repeat_forallb n :
+  forallb negb (repeat false n) = true.
+Proof.
+  induction n as [| ? IHn]; [reflexivity|cbn; apply IHn].
+Qed.
+
+(* A single instruction from a program is a subprogram of the full program *)
+Lemma sc_spec n i j (P : list (bsm_instr n)) x :
+  in_code j (i, P) ->
+  nth_error P (j - i) = Some x ->
+  (j, [x]) <sc (i, P).
+Proof.
+  intros H1 H2.
+  eexists (firstn (j - i) P), (skipn (j - i + 1) P).
+  split.
+  - cbn. 
+    replace (j - i + 1) with (S (j - i)) by lia.
+    now rewrite firstn_skipn_middle.
+  - cbn in H1.
+    rewrite firstn_length_le; [|lia].
+    rewrite Nat.add_sub_assoc; [|lia].
+    now rewrite Nat.add_comm, Nat.add_sub.
+Qed.
+
+(* BSM cast definition and lemmas *)
+Definition BSM_cast {n} (P : list (bsm_instr n)) {m} (E : n = m) : list (bsm_instr m).
+Proof. subst m. exact P. Defined.
+
+Lemma BSM_cast_length {n} (P : list (bsm_instr n)) {m} (E : n = m) :
+  length (BSM_cast P E) = length P.
+Proof.
+  destruct E. cbn. reflexivity.
+Qed.
+
+Lemma BSM_cast_spec {n m} i (P : list (bsm_instr n)) (E : n = m) j v k w :
+   sss.sss_compute (@bsm_sss _) (i, P) (j, v) (k, w) <-> sss.sss_compute (@bsm_sss _) (i, BSM_cast P E) (j, Vector.cast v E) (k, Vector.cast w E).
+Proof.
+  destruct E. cbn. now rewrite !cast_eq_refl.
 Qed.
 
 
-Lemma pos_right_left {n m} p q :
-@pos_left n m p <> @pos_right n m q.
+(* ---SBTM Simulation--- *)
+
+Definition complete_encode (Σ : finType) n (t : Vector.t (tape Σ) n) : SBTMNotations.tape:=
+  HaltTM_1_to_SBTM_HALT.encode_tape ((encode_tape' (Vector.nth (mTM_to_TM.enc_tape [] t) Fin0))).
+
+Lemma SBTM_complete_simulation n Σ (M : TM Σ n) :
+  {M' : SBTM &
+     {q_start : SBTMNotations.state M' |
+        (forall q t t' t'', TM.eval M (TM.start M) t q t' -> 
+          SBTM_facts.almost_eq_tape t'' (complete_encode t) ->
+        (exists k q' t''', SBTM.steps M' k (q_start, t'') = Some (q', t''') /\
+        SBTM.steps M' (S k) (q_start, t'') = None /\
+        SBTM_facts.almost_eq_tape t''' (complete_encode t'))) /\
+        (forall t, (exists k , SBTM.steps M' k (q_start, complete_encode t) = None) -> (exists q' t', TM.eval M (TM.start M) t q' t'))}}.
 Proof.
-induction n; cbn.
-- inversion p.
-- eapply (Fin.caseS' p).
-  + cbn. congruence.
-  + cbn. intros ? ? % pos_nxt_inj. firstorder.
+  destruct (TM_sTM_simulation M) as (M1 & Hf1 & Hb1).
+  destruct (binary_simulation M1) as (M2 & Hf2 & Hb2).
+  destruct (SBTM_simulation M2) as [M3 [q_start [Hf3 Hb3]]].
+  eexists M3, q_start.
+  split.
+  - intros q t t' t'' H H0.
+    destruct (Hf1 _ _ _ H) as [q' H1].
+    destruct (Hf2 _ _ _ H1) as [q'' H2].
+    apply (Hf3 _ _ _ t'' H2 H0).
+  - clear Hf1 Hf2 Hf3.
+    intros t H.
+    apply Hb1.
+    apply Hb2.
+    apply Hb3.
+    apply H.
 Qed.
 
-Lemma pos_left_right {n m} p q :
-@pos_right n m q <> @pos_left n m p.
-Proof.
-induction n; cbn.
-- inversion p.
-- eapply (Fin.caseS' p).
-  + cbn. congruence.
-  + cbn. intros ? ? % pos_nxt_inj. firstorder.
-Qed.
-Local Hint Immediate pos_left_right pos_right_left : core.
 
-Lemma vec_change_app_left {X} (n m : nat) v1 v2 p x:
-  vec_change (@vec_app X n m v1 v2) (pos_left m p) x = vec_app (vec_change v1 p x) v2.
-Proof.
-  eapply vec_pos_ext. eapply pos_left_right_rect.
-  - intros. rewrite !vec_pos_app_left.
-    destruct (pos_eq_dec p p0).
-    + subst. rewrite vec_change_eq. 2: reflexivity. now rewrite vec_change_eq.
-    + rewrite vec_change_neq. 2: intros ? % pos_left_inj; congruence.
-      rewrite vec_pos_app_left. rewrite vec_change_neq; auto.
-  - intros p0. rewrite !vec_pos_app_right. rewrite vec_change_neq; auto. now rewrite vec_pos_app_right.
-Qed.
+(* ---Extend BSM--- *)
 
-Lemma vec_app_inj {X} (n m : nat) v1 v2 v2' :
-  @vec_app X n m v1 v2 = vec_app v1 v2' -> v2 = v2'.
-Proof.
-  induction v1.
-  - now rewrite !vec_app_nil.
-  - rewrite !vec_app_cons. intros. eapply IHv1.
-    now eapply (f_equal (@vec_tail _ _)) in H.
-Qed.
+(* Lift instructions to more stacks *)
+Definition bsm_addstracks' n m (P : bsm_instr n) : (bsm_instr (m + n)) :=
+  (fun x => match x with
+  | bsm_pop x c1 c2 => bsm_pop (pos_right m x) c1 c2
+  | bsm_push x b => bsm_push (pos_right m x) b end) P.
 
+Definition bsm_addstacks n m (P : list (bsm_instr n)) : list (bsm_instr (m + n)):=
+map (@bsm_addstracks' n m) P.
+
+(* Lift single step *)
 Lemma BSM_addstacks_step n m (P : bsm_instr n) j v o v' v'' :
    (bsm_sss P (j, v) (o, v') <-> bsm_sss (@bsm_addstracks' n m P) (j, vec_app v'' v) (o, vec_app v'' v')).
 Proof.
@@ -294,6 +502,17 @@ Proof.
   - destruct st2. econstructor.  1: eapply BSM_addstacks_step'.  1: exact H1. eapply IHk, H2.
 Qed.
 
+(* Use sss_compute instead of sss_steps*)
+Lemma BSM_addstacks'' n i (P : list (bsm_instr n)) m j v o v' v'' :
+  sss_compute (bsm_sss (n := n)) (i, P) (j, v) (o, v') -> sss_compute (bsm_sss (n := m + n)) (i, (@bsm_addstacks n m P)) (j, vec_app v'' v) (o, vec_app v'' v').
+Proof.
+  intros H.
+  destruct H as [k H].
+  exists k.
+  apply BSM_addstacks'.
+  apply H.
+Qed.
+
 Lemma BSM_addstacks_bwd' n i (P : list (bsm_instr n)) m k j v v'' out :
   sss_steps (bsm_sss (n := m + n)) (i, (@bsm_addstacks n m P)) k (j, vec_app v'' v) out -> exists o v', out = (o, vec_app v'' v') /\ sss_steps (bsm_sss (n := n)) (i, P) k (j, v) (o, v').
 Proof.
@@ -320,389 +539,1084 @@ Proof.
     cbn in *. unfold bsm_addstacks in H2. rewrite length_map in H2. exact H2.
 Qed.
 
+(* Lifting a program does not change length *)
+Lemma bsm_length m n (P : list (bsm_instr n)):
+  length (bsm_addstacks m P) = length P.
+Proof.
+    destruct P as [| ? P]; [reflexivity |].
+    cbn.
+    now rewrite length_map.
+Qed.
+
+(* ---BSM encoding--- *)
+
+(* Encode tape vector on 5 BSM stacks.
+   0: Truncation stack
+   1: left of the current symbol
+   2: current symbol
+   3: right of the current symbol
+   5: Unconditional jump stack
+ *)
 Definition encode_bsm (Σ : finType) n (t : Vector.t (tape Σ) n) :=
-  enc_tape (complete_encode t).
+let t' := (SBTM_facts.truncate_tape (complete_encode t)) in 
+let t'' := (SBTM_HALT_to_HaltBSM.encode_tape t') in
+  vec_app [|[]|] t''.
+
+
 Arguments encode_bsm {_ _} _, _ {_} _.
 
 Arguments encode_tapes : simpl never.
 
-Lemma encode_bsm_nil (Σ : finType) n   :
-  { '(str2, n') | forall (t : Vector.t (tape Σ) n), (encode_bsm Σ (niltape ::: t))@[Fin2] =  str2 ++ (skipn n' ((encode_bsm Σ t)@[Fin2]))}.
+(* encode_symbol produces lists of length 2*)
+Lemma encode_length  l : (| flat_map encode_symbol l |) = 2 * (| l |).
 Proof.
-  eexists ((encode_sym _ ++ true :: false :: encode_sym _ ++ true :: false :: encode_sym _), _). intros t. cbn.
-  rewrite skipn_app'. 2: now rewrite length_encode_sym.
-  assert (Hreorder : forall l1 l2 l3 l4,
+  induction l; [reflexivity| ].
+  cbn in *.
+  lia.
+Qed.
+
+(* flat_map encode_symbol ends on true or is empty*)
+Lemma encode_symbol_spec l1 :
+  (exists l2, flat_map encode_symbol l1 = l2 ++ [true]) \/ l1 = [].
+Proof.
+  induction l1 as [ | a l1 IHl1].
+  - right. reflexivity.
+  - destruct IHl1 as [[l2 IHl1] | IHl1]; left.
+    + exists (a :: true :: l2).
+      cbn in *.
+      now rewrite IHl1.
+    + exists [a].
+      now rewrite IHl1.
+Qed.
+
+(* Reverse, remove false prefix, reverse does the same as truncate function*)
+Lemma trunc_spec l:
+  rev (remove_leading_falses (rev l)) = SBTM_facts.truncate l.
+Proof.
+  induction l as [| a l IHl]; [ now reflexivity |].
+  destruct a; cbn; [now rewrite <- IHl, remove_leading_falses_dist, rev_unit |].
+  destruct (leading_false_spec (rev l)) as [x [[x0 H] | H]].
+  - rewrite H in IHl.
+    rewrite H, <- app_assoc, <- app_comm_cons, remove_leading_falses_dist, <- IHl.
+    assert (E := true_not_repeat_false x x0).
+    rewrite <- rev_forallb in E.
+    rewrite <- H, rev_involutive in E.
+    now rewrite E, remove_leading_falses_dist, <- rev_unit, <- app_assoc, app_comm_cons.
+  - rewrite H, <- repeat_cons, <- IHl.
+    assert (H1 := repeat_forallb x).
+    rewrite <- H, rev_forallb in H1.
+    rewrite H1.
+    simpl.
+    now rewrite remove_leading_falses_spec_false_only.
+Qed.
+        
+(* Truncate does not have an effect because encode_symbol always ends on true*)
+Lemma truncate_irrel l:
+  SBTM_facts.truncate (flat_map encode_symbol l) = flat_map encode_symbol l.
+Proof.
+  destruct (encode_symbol_spec l) as [[l2 H] | H]; [| now rewrite H].
+  rewrite H, <- trunc_spec, rev_unit.
+  simpl.
+  now rewrite rev_involutive.
+Qed.
+
+(* truncate_irrel applied to an encoded BSM stack configuration *)
+Lemma truncate_irrel_encoding (Σ : finType) n (t: vec (tape Σ) n) :
+  (encode_bsm t)@[Fin3] = (vec_app [|[]|] (SBTM_HALT_to_HaltBSM.encode_tape (complete_encode t)))@[Fin3].
+Proof.
+  unfold encode_bsm.
+  simpl.
+  now rewrite truncate_irrel.
+Qed.
+
+Lemma encode_bsm_nil (Σ : finType) n   :
+  { '(str2, n') | forall (t : Vector.t (tape Σ) n), (encode_bsm Σ (niltape ::: t))@[Fin3] =  str2 ++ (skipn n' ((encode_bsm Σ t)@[Fin3]))}.
+Proof.
+  eexists (flat_map encode_symbol (encode_sym _ ++ true :: false :: encode_sym _ ++ true :: false :: encode_sym _), _). intros t.
+  cbn.
+  rewrite !truncate_irrel.
+  rewrite !flat_map_app.
+  rewrite skipn_app'; [|now rewrite encode_length, length_encode_sym]. 
+  rewrite <- !flat_map_app. 
+  f_equal.
+  assert ( Hreorder : forall l1 l2 l3 l4,
   l1 ++ true :: false :: l2 ++ true :: false :: l3 ++ true :: l4 =
-  (l1 ++ true :: false :: l2 ++ true :: false :: l3) ++ true :: l4).
+  (l1 ++ true :: false :: l2 ++ true :: false :: l3) ++ true :: l4). 
   { intros. now repeat (rewrite <- app_assoc; cbn). }
   apply Hreorder.
 Qed.
 
-Definition strpush_common_short (Σ : finType) (s b : Σ) :=
-encode_sym
+(* Function definitions to improve performance*)
+Definition encoding_func' (Σ : finType)  x :=
   (projT1
      (projT2
         (FinTypes.finite_n
            (finType_CS (boundary + sigList (EncodeTapes.sigTape Σ)))))
-     (inl START)) ++
+     x).
+
+Definition encoding_func (Σ : finType) x :=
+encode_sym (@encoding_func' Σ x).
+
+Definition strpush_common_short (Σ : finType) (s b : Σ) :=
+flat_map encode_symbol ((@encoding_func Σ (inl START)) ++
 true
 :: false
-   :: encode_sym
-        (projT1
-           (projT2
-              (FinTypes.finite_n
-                 (finType_CS (boundary + sigList (EncodeTapes.sigTape Σ)))))
-           (inr sigList_cons)) ++
+   :: @encoding_func Σ (inr sigList_cons) ++
       true
       :: false
-         :: encode_sym
-              (projT1
-                 (projT2
-                    (FinTypes.finite_n
-                       (finType_CS
-                          (boundary + sigList (EncodeTapes.sigTape Σ)))))
-                 (inr (sigList_X (EncodeTapes.LeftBlank false)))) ++
+         :: @encoding_func Σ (inr (sigList_X (EncodeTapes.LeftBlank false))) ++
             true
             :: false
-               :: encode_sym
-                    (projT1
-                       (projT2
-                          (FinTypes.finite_n
-                             (finType_CS
-                                (boundary + sigList (EncodeTapes.sigTape Σ)))))
-                       (inr (sigList_X (EncodeTapes.MarkedSymbol b)))).
+               :: @encoding_func Σ (inr (sigList_X (EncodeTapes.MarkedSymbol b)))).
+
 
 Definition strpush_common (Σ : finType) (s b : Σ) :=
 strpush_common_short s b ++
+            flat_map encode_symbol(
                   true
-                  :: false :: nil.
+                  :: false :: nil).
+
 
 Definition strpush_zero (Σ : finType) (s b : Σ) :=
   strpush_common s b ++
-                      encode_sym
-                          (projT1
-                             (projT2
-                                (FinTypes.finite_n
-                                   (finType_CS
-                                      (boundary +
-                                       sigList (EncodeTapes.sigTape Σ)))))
-                             (inr (sigList_X (EncodeTapes.RightBlank false)))).
+        flat_map encode_symbol (
+                     @encoding_func Σ (inr (sigList_X (EncodeTapes.RightBlank false)))).
+
 
 Lemma encode_bsm_at0 (Σ : finType) n (t : Vector.t (tape Σ) n) :
    (encode_bsm Σ t) @[Fin0] = [].
-Proof.
-  reflexivity.
-Qed.
+Proof. reflexivity. Qed.
 
-Lemma encode_bsm_at1 (Σ : finType) n :
-   forall (t : Vector.t (tape Σ) n), (encode_bsm Σ t) @[Fin1] = [false].
-Proof.
-  intros t.
-  reflexivity.
-Qed.
+Lemma encode_bsm_at1 (Σ : finType) n (t : Vector.t (tape Σ) n) :
+   (encode_bsm Σ t) @[Fin1] = [].
+Proof. reflexivity. Qed.
 
-Lemma encode_bsm_at3 (Σ : finType) n (t : Vector.t (tape Σ) n) :
-   (encode_bsm Σ t) @[Fin3] = [].
-Proof.
-  reflexivity.
-Qed.
+Lemma encode_bsm_at2 (Σ : finType) n :
+   forall (t : Vector.t (tape Σ) n), (encode_bsm Σ t) @[Fin2] = [true].
+Proof. reflexivity. Qed.
+
+Lemma encode_bsm_at4 (Σ : finType) n (t : Vector.t (tape Σ) n) :
+   (encode_bsm Σ t) @[Fin4] = [].
+Proof. reflexivity. Qed.
 
 Lemma encode_bsm_zero (Σ : finType) s b :
-  { n' | forall n(t : Vector.t (tape Σ) n), (encode_bsm Σ (encNatTM s b 0 ::: t)) @[Fin2] = strpush_zero s b ++ (skipn n' ((encode_bsm Σ t)@[Fin2]))}.
+  { n' | forall n(t : Vector.t (tape Σ) n), (encode_bsm Σ (encNatTM s b 0 ::: t)) @[Fin3] = strpush_zero s b ++ (skipn n' ((encode_bsm Σ t)@[Fin3]))}.
 Proof.
   eexists _. intros ? t. cbn.
-  rewrite skipn_app'. 2: now rewrite length_encode_sym.
+  rewrite !truncate_irrel, !flat_map_app.
+  rewrite skipn_app'; [ | now rewrite encode_length, length_encode_sym].
   unfold strpush_zero, strpush_common, strpush_common_short.
   assert (Hreorder : forall l1 l2 l3 l4 l5 l6,
     l1 ++ true :: false :: l2 ++ true :: false :: l3 ++ true :: false :: l4 ++ true :: false :: l5 ++ true :: l6 =
     (((l1 ++ true :: false :: l2 ++ true :: false :: l3 ++ true :: false :: l4) ++ [true; false]) ++ l5) ++ true :: l6).
   { intros. now repeat (rewrite <- app_assoc; cbn). }
+  rewrite <- !flat_map_app.
+  f_equal.
   apply Hreorder.
 Qed.
 
 Definition strpush_succ (Σ : finType) (s b : Σ) :=
 strpush_common s b ++
-                     encode_sym
-                          (projT1
-                             (projT2
-                                (FinTypes.finite_n
-                                   (finType_CS
-                                      (boundary +
-                                       sigList (EncodeTapes.sigTape Σ)))))
-                             (inr (sigList_X (EncodeTapes.UnmarkedSymbol s)))).
+        flat_map encode_symbol (
+                    encoding_func (inr (sigList_X (EncodeTapes.UnmarkedSymbol s)))).
 
 Lemma encode_tapes_cons {sig n} t (ts : tapes sig n) : encode_tapes (t ::: ts) = sigList_cons :: map sigList_X (encode_tape t) ++ encode_tapes ts.
 Proof. reflexivity. Qed.
 
 Lemma encode_bsm_succ (Σ : finType) n m s b (t : Vector.t (tape Σ) n) :
-      (encode_bsm Σ (encNatTM s b (S m) ::: t)) @[Fin2] = strpush_succ s b ++ (skipn (length (strpush_common_short s b)) ((encode_bsm Σ (encNatTM s b m ::: t))@[Fin2])).
+      (encode_bsm Σ (encNatTM s b (S m) ::: t)) @[Fin3] = strpush_succ s b ++ (skipn (length (strpush_common_short s b)) ((encode_bsm Σ (encNatTM s b m ::: t))@[Fin3])).
 Proof.
-  cbn. rewrite (encode_tapes_cons (encNatTM s b m)). cbn.
-  assert (Hskip : forall n l1 l2 l3 l4 l5,
-    n = length (l1 ++ true :: false :: l2 ++ true :: false :: l3 ++ true :: false :: l4) ->
-    skipn n (l1 ++ true :: false :: l2 ++ true :: false :: l3 ++ true :: false :: l4 ++ l5) = l5).
-  { intros ?????? ->. repeat (rewrite skipn_app_app; cbn). now rewrite skipn_app'. }
-  rewrite Hskip. 2: { reflexivity. }
-  unfold strpush_succ, strpush_common, strpush_common_short.
-  assert (Hreorder : forall l1 l2 l3 l4 l5 l6,
-    l1 ++ true :: false :: l2 ++ true :: false :: l3 ++ true :: false :: l4 ++ true :: false :: l5 ++ true :: l6 =
-    (((l1 ++ true :: false :: l2 ++ true :: false :: l3 ++ true :: false :: l4) ++ [true; false]) ++ l5) ++ true :: l6).
+  rewrite !truncate_irrel_encoding.
+  rewrite <- !vec_pos_spec.
+  rewrite !vec_pos_app_right.
+  cbn.
+  set (X := map _). set (Y := encode_sym _).
+  replace X with (map (@encoding_func' Σ)) by reflexivity.
+  replace Y with (encode_sym (@encoding_func' Σ (inl START))) by reflexivity.
+  rewrite (encode_tapes_cons (encNatTM s b m)). cbn.
+  assert (Happ_assoc : forall l1 l2 l3 l4 l5,
+    l1 ++ true :: false :: l2 ++ true :: false :: l3 ++ true :: false :: l4 ++ true :: l5 =
+    (l1 ++ true :: false :: l2 ++ true :: false :: l3 ++ true :: false :: l4) ++ true :: l5).
   { intros. now repeat (rewrite <- app_assoc; cbn). }
-  apply Hreorder.
+  rewrite Happ_assoc.
+  rewrite !flat_map_app.
+  rewrite skipn_app'.
+  - unfold strpush_succ, strpush_common, strpush_common_short.
+    rewrite <- !flat_map_app.
+    f_equal.
+    assert( Hreorder : forall l1 l2 l3 l4 l5 l6,
+    l1 ++ true :: false :: l2 ++ true :: false :: l3 ++ true :: false :: l4 ++ true :: false :: l5 ++ true :: l6 =
+    (((l1 ++ true :: false :: l2 ++ true :: false :: l3 ++ true :: false :: l4) ++ [true; false]) ++ l5) ++ true :: l6). {
+   intros. now repeat (rewrite <- app_assoc; cbn). }
+    apply Hreorder.
+  - rewrite length_app.
+    rewrite encode_length.
+    rewrite length_encode_sym.
+    unfold strpush_common_short.
+    rewrite flat_map_app.
+    rewrite length_app.
+    unfold encoding_func.
+    rewrite encode_length.
+    now rewrite length_encode_sym.
 Qed.
 
-Lemma BSM_complete_simulation' n Σ (M : TM Σ n) m i :
-{ P |
-      (forall q t t', TM.eval M (TM.start M) t q t' ->
-       forall v'', BSM.eval (m + (4)) (i, P) (i, Vector.append v'' ((encode_bsm t))) (i + length P, Vector.append v'' ((encode_bsm t')))) /\
-      (forall t v'', (exists out, BSM.eval (m + (4)) (i, P) (i, Vector.append v'' ((encode_bsm t))) out) -> (exists q' t', TM.eval M (TM.start M) t q' t'))}.
+
+(* ---Truncation simulation--- *)
+
+Section Truncation_Construction.
+
+  (* STACK is the stack to perform truncation on. STACK is different from the truncation and the empty stack. *)
+  Context (i : nat) (STACK : Fin.t 5) (STACK_NEQ_FIN4 : STACK <> Fin4) (STACK_NEQ_FIN0 : STACK <> Fin0).
+
+  Definition TRUNC_length := 12.
+  Definition END := i + TRUNC_length.
+
+  (* Performs truncation on one stack *)
+  #[local] Definition TRUNC : list (bsm_instr 5) :=
+    let JMP := fun i => POP Fin4 i i in
+    (* i + 0 *) POP STACK (i + 3) (i + 5) ::
+    (* i + 1 *) PUSH Fin0 true ::
+    (* i + 2 *) JMP (i + 0) ::
+    (* i + 3 *) PUSH Fin0 false ::
+    (* i + 4 *) JMP (i + 0) ::
+
+    (* i + 5 *) POP Fin0 (i + 5) END ::
+    (* i + 6 *) PUSH Fin0 true ::
+
+    (* i + 7 *) POP Fin0 (i + 10) END ::
+    (* i + 8 *) PUSH STACK true ::
+    (* i + 9 *) JMP (i + 7) ::
+    (* i + 10 *) PUSH STACK false ::
+    (* i + 11 *) JMP (i + 7) :: [].
+
+
+  (* Specifies one traversal of the first loop (i to (i + 4))*)
+  #[local] Lemma Truncation_first_loop_single a v v1:
+    vec_pos v Fin4 = [] ->
+    vec_pos v STACK = a :: v1 ->
+    (i, TRUNC) // (i, v) ->> 
+    (i, vec_change (vec_change v STACK v1) Fin0 (a :: vec_pos v Fin0)).
+  Proof using STACK_NEQ_FIN0 STACK_NEQ_FIN4.
+    unfold TRUNC.
+    intros H1 H2.
+    destruct a.
+    - bsm sss POP one with STACK (i + 3) (i + 5) v1.
+      bsm sss PUSH with Fin0 true.
+      bsm sss POP empty with Fin4 (i + 0) (i + 0).
+      + repeat rewrite vec_change_neq; easy.
+      + rewrite Nat.add_0_r.
+        bsm sss stop.
+        rewrite vec_change_neq; easy.
+    - bsm sss POP zero with STACK (i + 3) (i + 5) v1.
+      bsm sss PUSH with Fin0 false.
+      replace (1 + ( i + 3)) with (i + 4) by lia.
+      bsm sss POP empty with Fin4 (i + 0) (i + 0).
+      + apply sc_spec; cbn; [lia |now replace (i + 4 - i) with 4 by lia].
+      + repeat rewrite vec_change_neq; easy.
+      + rewrite Nat.add_0_r.
+        bsm sss stop.
+        rewrite vec_change_neq; easy.
+  Qed.
+
+  (* Specifies traversal of the first loop (i to (i + 4))*)
+  #[local] Lemma Truncation_first_loop v v0 v1:
+    vec_pos v Fin4 = [] ->
+    vec_pos v Fin0 = v0 ->
+    vec_pos v STACK = v1 ->
+    (i, TRUNC) // (i, v) ->> (i, 
+    vec_change (vec_change v STACK []) Fin0 (rev v1 ++ v0)).
+  Proof using STACK_NEQ_FIN0 STACK_NEQ_FIN4.
+    revert v0 v.
+    induction v1 as [|a v1 IHv1]; intros v2 v H1 H2 H3.
+    - simpl. exists 0. rewrite <- H3. rewrite vec_change_same. rewrite <- H2. rewrite vec_change_same. constructor.
+    - eapply sss_compute_trans.
+      + apply Truncation_first_loop_single; [easy | now apply H3].
+      + enough (E :(vec_change (vec_change (vec_change (vec_change v STACK v1) Fin0 (a :: vec_pos v Fin0)) STACK []) Fin0(rev v1 ++ a :: v2)) = (vec_change (vec_change v STACK []) Fin0 (rev (a :: v1) ++ v2))).
+        * rewrite <- E, <- H2.
+          apply IHv1; now autorewrite with vec_simpl.
+        * rewrite <- H2.
+          rewrite vec_change_comm; [|easy].
+          rewrite vec_change_idem.
+          rewrite vec_change_comm; [|easy].
+          rewrite vec_change_idem.
+          simpl.
+          rewrite <- app_assoc.
+          now rewrite <- app_comm_cons.
+  Qed.
+
+  (* Specifies traversal from first to second loop (i to (i + 5))*)
+  #[local] Lemma Truncation_first_to_second v:
+    vec_pos v Fin4 = [] ->
+    vec_pos v STACK = [] ->
+    (i, TRUNC) // (i, v) ->> (i + 5, v).
+  Proof.
+    unfold TRUNC.
+    intros H1 H2.
+    bsm sss POP empty with STACK (i + 3) (i + 5).
+    bsm sss stop.
+  Qed.
+
+  (* Specifies traversal of second loop ((i + 5) and (i + 6)) if STACK contains a false prefix *)
+  #[local] Lemma Truncation_second_loop_repeat_false n v v0:
+    vec_pos v Fin4 = [] ->
+    vec_pos v Fin0 = (repeat false n) ++ v0 ->
+    vec_pos v STACK = [] ->
+    (i, TRUNC) // (i + 5, v) ->> (i + 5, vec_change v Fin0 v0).
+  Proof using STACK_NEQ_FIN0.
+    revert v.
+    induction n as [|n IHn]; intros v H0 H1 H2.
+    - exists 0. cbn in H1. rewrite <- H1. rewrite vec_change_same. constructor.
+    - eapply sss_compute_trans.
+      + unfold TRUNC.
+        bsm sss POP zero with Fin0 (i + 5) (END) (repeat false n ++ v0).
+        bsm sss stop.
+      + enough (H :vec_change (vec_change v Fin0 (repeat false n ++ v0)) Fin0 v0 = vec_change v Fin0 v0).
+        * rewrite <- H.
+          apply IHn; now autorewrite with vec_simpl.
+        * now rewrite vec_change_idem.
+  Qed.
+
+  (* Specifies traversal of second loop ((i + 5) and (i + 6)) if STACK starts with true *)
+  #[local] Lemma Truncation_second_loop_true v v0:
+    vec_pos v Fin4 = [] ->
+    vec_pos v Fin0 = true :: v0 ->
+    vec_pos v STACK = [] -> 
+    (i, TRUNC) // (i + 5, v) ->> (i + 7, v).
+  Proof using STACK_NEQ_FIN0 STACK_NEQ_FIN4.
+    unfold TRUNC.
+    intros H H0 H1.
+    bsm sss POP one with Fin0 (i + 5) (END) v0.
+    bsm sss PUSH with Fin0 true.
+    - apply sc_spec; [cbn; lia| now replace (1 + (i + 5) - i) with 6 by lia].
+    - bsm sss stop.
+      f_equal; [lia|].
+      rewrite vec_change_idem.
+      rewrite vec_change_eq; [|easy].
+      rewrite <- H0.
+      now rewrite vec_change_same.
+  Qed.
+
+  (* Specifies traversal of second loop ((i + 5) and (i + 6)) if STACK is empty *)
+  #[local] Lemma Truncation_second_loop_empty v:
+    vec_pos v Fin0 = [] ->
+    vec_pos v STACK = [] ->
+    vec_pos v Fin4 = [] ->
+    (i, TRUNC) // (i + 5, v) ->> (END, v).
+  Proof.
+    unfold TRUNC.
+    intros H H0 H1.
+    bsm sss POP empty with Fin0 (i + 5) (END).
+    bsm sss stop.
+  Qed.
+
+  (* Specifies one traversal of third loop ((i + 7) to (i + 11)) *)
+  #[local] Lemma Truncation_third_loop_single a v v0:
+    vec_pos v Fin0 = a :: v0 ->
+    vec_pos v Fin4 = [] ->
+    (i, TRUNC) // (i + 7, v) ->> (i + 7, vec_change (vec_change v Fin0 v0) STACK (a :: vec_pos v STACK)).
+  Proof using STACK_NEQ_FIN0 STACK_NEQ_FIN4.
+    unfold TRUNC.
+    intros H H0.
+    destruct a.
+    - bsm sss POP one with Fin0 (i + 10) (END) v0.
+      bsm sss PUSH with STACK true.
+      bsm sss POP empty with Fin4 (i + 7) (i + 7); [now autorewrite with vec_simpl|].
+      bsm sss stop.
+      now autorewrite with vec_simpl.
+    - bsm sss POP zero with Fin0 (i + 10) (END) v0.
+      bsm sss PUSH with STACK false.
+      bsm sss POP empty with Fin4 (i + 7) (i + 7); [| now autorewrite with vec_simpl |].
+      + apply sc_spec; [cbn; lia | now replace (1 + (i + 10) - i) with 11 by lia].
+      + bsm sss stop.
+        now autorewrite with vec_simpl.
+  Qed.
+
+  (* Specifies traversal of third loop ((i + 7) to (i + 11)) *)
+  #[local] Lemma Truncation_third_loop v v0 v1:
+    vec_pos v Fin4 = [] ->
+    vec_pos v Fin0 = v0 ->
+    vec_pos v STACK = v1 ->
+    (i, TRUNC) // (i + 7, v) ->> (i + 7,
+    vec_change (vec_change v STACK (rev v0 ++ v1)) Fin0 []).
+  Proof using STACK_NEQ_FIN0 STACK_NEQ_FIN4.
+    revert v v1.
+    induction v0 as [|a v0 IHv0].
+    - intros v l H0 H1 H2. cbn. exists 0. rewrite <- H2, vec_change_same, <- H1, vec_change_same. now constructor.
+    - intros v l H0 H1 H2.
+      eapply sss_compute_trans.
+      + apply Truncation_third_loop_single; [|easy].
+        now apply H1.
+      + enough (H :vec_change (vec_change (vec_change (vec_change v Fin0 v0) STACK
+  (a :: vec_pos v STACK)) STACK (rev v0 ++ a :: l))
+  Fin0 [] = vec_change (vec_change v STACK (rev (a :: v0) ++ l))
+  Fin0 []).
+      * rewrite <- H, H2.
+        apply IHv0; now autorewrite with vec_simpl; easy.
+      * rewrite vec_change_idem.
+        rewrite vec_change_comm; [|easy].
+        rewrite vec_change_idem.
+        rewrite vec_change_comm; [|easy].
+        simpl.
+        now rewrite <- app_assoc.
+  Qed.
+
+  (* Specifies traversal from (i + 7) to END*)
+  #[local] Lemma Truncation_spec_final v:
+    vec_pos v Fin4 = [] ->
+    vec_pos v Fin0 = [] ->
+    (i, TRUNC) // (i + 7, v) ->> (END, v).
+  Proof.
+    unfold END, TRUNC, TRUNC_length.
+    intros H H0.
+    bsm sss POP empty with Fin0 (i + 10) (i + 12); [|bsm sss stop].
+    apply sc_spec; [cbn; lia |  now replace (i + 7 - i) with 7 by lia].
+  Qed.
+
+  (* Apply truncate to STACK *)
+  Definition trunc_stack v := vec_change v STACK (SBTM_facts.truncate (Vector.nth v STACK)).
+
+  (* Specifes the truncation of STACK*)
+  Lemma Truncation_spec_END v:
+    vec_pos v Fin4 = [] ->
+    vec_pos v Fin0 = [] ->
+    (i, TRUNC) // (i, v) ->> 
+    (END,vec_change v STACK (rev (remove_leading_falses (rev (vec_pos v STACK))))).
+  Proof using STACK_NEQ_FIN0 STACK_NEQ_FIN4.
+    intros I1 I2. 
+    eapply sss_compute_trans.
+    2: eapply sss_compute_trans.
+    - apply Truncation_first_loop; now autorewrite with vec_simpl.
+    - apply Truncation_first_to_second; now autorewrite with vec_simpl.
+    - destruct (leading_false_spec (rev (vec_pos v STACK))) as [n [[l E]|E]].
+      + eapply sss_compute_trans.
+        2: eapply sss_compute_trans.
+        3: eapply sss_compute_trans.
+        4: eapply sss_compute_trans.
+        * eapply Truncation_second_loop_repeat_false; autorewrite with vec_simpl; [easy | | easy].
+        rewrite E. now rewrite app_assoc.
+        * eapply Truncation_second_loop_true; autorewrite with vec_simpl; [easy | | easy].
+        now rewrite <- app_comm_cons.
+        * apply Truncation_third_loop; now autorewrite with vec_simpl.
+        * apply Truncation_spec_final; now autorewrite with vec_simpl.
+        * bsm sss stop. f_equal.
+          rewrite !vec_change_idem.
+          rewrite vec_change_comm; [|easy].
+          rewrite vec_change_idem.
+          rewrite vec_change_comm; [|easy].
+          rewrite vec_change_idem.
+          rewrite vec_change_comm; [|easy].
+          rewrite E.
+          rewrite remove_leading_falses_spec.
+          rewrite <- I2.
+          rewrite vec_change_same.
+          rewrite I2.
+          now rewrite !app_nil_r.
+      + eapply sss_compute_trans.
+        2: eapply sss_compute_trans.
+        * eapply Truncation_second_loop_repeat_false; autorewrite with vec_simpl; [easy | | easy].
+          now rewrite E.
+        * apply Truncation_second_loop_empty; now autorewrite with vec_simpl.
+        * bsm sss stop. f_equal.
+          rewrite vec_change_idem.
+          rewrite vec_change_comm; [|easy].
+          rewrite vec_change_same.
+          rewrite E.
+          now rewrite remove_leading_falses_spec_false_only.
+  Qed.
+
+End Truncation_Construction.
+
+(* Define truncation program. Use TRUNC on stacks 1 and 3*)
+Definition TRUNC_PROG i: list (bsm_instr 5) :=
+  TRUNC i Fin1 ++ TRUNC (i + TRUNC_length) Fin3.
+
+(* Apply trunc_stack to stacks 1 and 3*)
+Definition trunc_conf (v : vec (list bool) 5) :=
+  trunc_stack Fin3 (trunc_stack Fin1 v).
+  
+(* TRUNC_PROG truncates a stack configuration*)
+Lemma TRUNC_PROG_spec i v:
+  vec_pos v Fin4 = [] ->
+  vec_pos v Fin0 = [] ->
+  (i, TRUNC_PROG i) // (i, v) ->> (i + (|TRUNC_PROG i|), trunc_conf v).
 Proof.
-  destruct (KOSBTM_complete_simulation M) as (M1 & Hf1 & Hb1).
-  destruct (BSM_addstacks i (SIM M1 i) m ) as (M2 & Hl & Hf2 & Hb2).
-  exists M2. split.
-  - intros q t t' [q1 H % (SIM_computes i) ] % Hf1.
-    intros. eapply Hf2. eapply BSM_sss.eval_iff. split.
-    1: cbn [Fin.to_nat proj1_sig mult] in H.  1: rewrite !Nat.add_0_l, Nat.add_0_r in H.
-    1: rewrite <- Hl.  1: rewrite SIM_length.  1: rewrite Nat.mul_comm.  1: eapply H.
-    right. unfold fst, subcode.code_end, snd, fst. rewrite <- Hl. lia.
-  - intros t v'' (out & [[out1 out2] [Ho1 Ho2]% BSM_sss.eval_iff] % Hb2). eapply Hb1.
-    eapply SIM_term with (q := Fin.F1) in Ho2 .
-    2:{ cbn [Fin.to_nat proj1_sig mult]. rewrite !Nat.add_0_l, Nat.add_0_r. eapply Ho1. }
-    destruct Ho2 as (q' & t' & H1 & -> & H2). eauto.
+  intros I1 I2.
+  eapply sss_compute_trans;[| eapply sss_compute_trans].
+  - eapply subcode_sss_compute;[ | apply (@Truncation_spec_END i Fin1); easy].
+    eexists [], _.
+    split; [now reflexivity | simpl; lia]. 
+  - eapply subcode_sss_compute; [|apply (@Truncation_spec_END (i + TRUNC_length) Fin3)]; rewrite ?vec_change_neq; [eexists (TRUNC i Fin1), _; now split| easy| easy | easy | easy | easy | easy].
+  - bsm sss stop. cbn. unfold END, TRUNC_length.
+    f_equal; [lia|].
+    unfold trunc_conf, trunc_stack.
+    rewrite <- !vec_pos_spec.
+    rewrite !trunc_spec.
+    reflexivity.
 Qed.
 
-Lemma BSM_complete_simulation n Σ (M : TM Σ n) m  i :
-{ P |
+(* It does not matter if truncation is performed on the SBTM tape or simulated on the BSM stack configuration *)
+Lemma trunc_order t:
+  trunc_conf (vec_app [|[]|] (SBTM_HALT_to_HaltBSM.encode_tape t)) = vec_app [|[]|] (SBTM_HALT_to_HaltBSM.encode_tape (SBTM_facts.truncate_tape t)).
+Proof.
+  destruct t as [[l c] r].
+  now reflexivity.
+Qed.
+
+
+(* ---Inverse truncation--- *)
+
+(* Define inverse truncation program. To perform inverse truncation on a tape encoded by encode_bsm, one PUSH suffices. *)
+Definition INV_TRUNC_PROG := [ @PUSH 5 Fin1 false].
+
+Lemma INV_TRUNC_PROG_length : | INV_TRUNC_PROG | = 1.
+Proof. now cbn. Qed.
+
+(* INV_TRUNC_PROG performs inverse truncation on a tape encoded by encode_bsm *)
+Lemma INV_TRUNC_spec (n : nat) (Σ : finType) t i: 
+  (i, INV_TRUNC_PROG) // (i, encode_bsm t) ->> 
+  (i + 1 , vec_app [|[]|] (SBTM_HALT_to_HaltBSM.encode_tape (@complete_encode Σ n t))).
+Proof.
+  unfold INV_TRUNC_PROG.
+  bsm sss PUSH with Fin1 false.
+  + apply sc_spec; [cbn; lia | now replace (i - i) with 0 by lia].
+  + bsm sss stop.
+    unfold complete_encode.
+    cbn.
+    rewrite truncate_irrel.
+    f_equal.
+    lia. 
+Qed.
+
+
+(* ---Simulation Program--- *)
+
+(* Define the full simulation program. 
+  1. Perform inverse truncation
+  2. Program from SBTM to BSM (extended to 5 stacks)
+  3. Perform truncation
+ *)
+Definition FULL_PROG M1 q1 i := 
+                        INV_TRUNC_PROG ++ 
+                        bsm_addstacks 1 (P M1 q1 (i + 1)) ++
+                        TRUNC_PROG (i + 1 + (|P M1 q1 (i + 1)|)).
+                        
+(* If a program never pushes to STACK, then STACK remains empty after a step *)
+Lemma Step_empty_spec i j n t v M M' M'' STACK:
+    in_code j (i + (|M''|), M) ->
+    vec_pos v STACK = [] ->
+    Forall 
+    (fun instr => match instr with 
+                    | PUSH s _ => s <> STACK
+                    | _ => True
+                    end) M ->
+    sss_step (bsm_sss (n:=5)) (i, M''++ M ++ M') (j, v) (n, t) ->
+    vec_pos t STACK = [].
+Proof.
+  intros H H0 H1 H2.
+  assert (H3:(i + (| M'' |), M) <sc ((i, M'' ++ M ++ M'))) by auto.
+  replace j with (fst (j,v)) in H by easy.
+  destruct (sss_step_supcode H3 H H2) as [? [l [i' [? [? [H2A [H2B H2C]]]]]]]. clear H2 H3.
+  injection H2A. injection H2B. intros H2 H3 H4 H5. clear H2A H2B.
+  rewrite Forall_nth in H1.
+  cbn in H.
+  assert (H6 : j - (i + (|M''|)) < |M|) by lia.
+  assert (H7 : j - ((i + (|M''|))) = |l|) by lia.
+  specialize (H1 _ (PUSH Fin0 true) H6).
+  rewrite H7, H4 in H1.
+  rewrite app_nth2 in H1; [|lia].
+  replace ((|l|) - (|l|)) with 0 in H1 by lia.
+  cbn in H1.
+  destruct i' eqn:I; [apply (POP_empty_spec' H0 H2C)|].
+  apply PUSH_spec in H2C.
+  destruct H2C as [_ H2C].
+  rewrite H2C.
+  rewrite vec_change_neq; [apply H0| easy].
+Qed.
+
+(* If every jump label in a program is either inside the program or at the first label behind the program,
+then this holds for each program counter after performing a step *)
+Lemma in_code_step_spec i j n t v M M' M'':
+  in_code j (i + (|M''|), M) ->
+  Forall 
+  (fun instr => match instr with 
+                  | POP _ k1 k2 => (in_code k1 (i + (|M''|), M) \/ k1 = i + (|M''|) + (|M|)) /\
+                                  (in_code k2 (i + (|M''|), M) \/ k2 = i + (|M''|) + (|M|))
+                  | _ => True
+                  end) M ->
+  sss_step (bsm_sss (n:=5)) (i, M'' ++ M ++ M') (j, v) (n, t) ->
+  (in_code n (i + (|M''|), M) \/ n = i + (|M''|) + (|M|)).
+Proof.
+  intros H H1 H2.
+  assert (H3:(i + (| M'' |), M) <sc ((i, M'' ++ M ++ M'))) by auto.
+  replace j with (fst (j,v)) in H by easy.
+  destruct (sss_step_supcode H3 H H2) as [? [l [i' [? [? [H2A [H2B H2C]]]]]]]. clear H2 H3.
+  injection H2A. injection H2B. intros H2 H3 H4 H5. clear H2A H2B.
+  rewrite Forall_nth in H1.
+  cbn in H.
+  assert (H6 : j - (i + (|M''|)) < |M|) by lia.
+  assert (H7 : j - ((i + (|M''|))) = |l|) by lia.
+  specialize (H1 _ (PUSH Fin0 true) H6).
+  rewrite H7, H4 in H1.
+  rewrite app_nth2 in H1; [|lia].
+  replace ((|l|) - (|l|)) with 0 in H1 by lia.
+  destruct i' as [m??| ] eqn:I.
+  + destruct (vec_pos v m) as [|b y] eqn:E;[|destruct b].
+      * apply POP_empty_spec in H2C;[|now apply E].
+        destruct H2C as [H2C _].
+        destruct H1 as [_ H1].
+        rewrite H2C.
+        rewrite <- H4 in H1.
+        apply H1.
+      * apply POP_true_spec with (v' := y) in H2C; [|now apply E].
+        destruct H2C as [H2C _].
+        rewrite H2C.
+        cbn. lia.          
+      * apply POP_false_spec with (v' := y) in H2C; [|now apply E].
+        destruct H2C as [H2C _].
+        destruct H1 as [H1 _].
+        rewrite H2C.
+        rewrite <- H4 in H1.
+        apply H1.
+    + apply PUSH_spec in H2C.
+      destruct H2C as [H2C _]. rewrite H2C.
+      cbn. lia.
+Qed.
+
+(* k either lies within the BSM program for SBTM M1 or is the first code label behind the program*)
+Definition in_code_or_exact_end k M1 q1 i := 
+  in_code k (i , bsm_addstacks 1 (P M1 q1 i)) \/
+    k = i + (| bsm_addstacks 1 (P M1 q1 i) |).
+
+(* in_code_or_exact_end holds for each POP of PROG *)
+Lemma PROG_JMP_spec M1 q1 i q:
+  Forall (fun instr : bsm_instr 4 =>
+    match bsm_addstracks' 1 instr with
+      | POP _ k1 k2 =>
+          @in_code_or_exact_end k1 M1 q1 (i + 1) /\
+          @in_code_or_exact_end k2 M1 q1 (i + 1)
+      | PUSH _ _ => True
+    end) (PROG M1 (i + 1) q).
+Proof.
+  assert (C := c_spec).
+  assert (U := SBTM_HALT_to_HaltBSM.state_number_length M1 q).
+  assert (N := SBTM_HALT_to_HaltBSM.state_map_length_spec M1).
+  assert (H1 : forall j, j < c -> @in_code_or_exact_end (j + encode_state M1 (i + 1) q) M1 q1 (i + 1)). {
+    unfold in_code_or_exact_end.
+    rewrite !bsm_length. cbn. rewrite length_map, length_app, length_flat_map_PROG_M. lia.
+  }
+  assert (H2 : forall j, j < 4 ->  @in_code_or_exact_end (j + (i + 1) + c * num_states M1) M1 q1 (i + 1)). {
+    unfold in_code_or_exact_end.
+    rewrite !bsm_length. cbn. rewrite length_map, length_app, length_flat_map_PROG_M. simpl. lia.
+  }
+  assert (H3 : forall q, (@in_code_or_exact_end (encode_state M1 (i + 1) q) M1 q1 (i + 1))). {
+    intros q'. unfold in_code_or_exact_end.
+    rewrite !bsm_length. cbn. rewrite length_map, length_app, length_flat_map_PROG_M. simpl. 
+    assert (H := state_number_length M1 q').
+    lia.
+  }
+  repeat apply Forall_cons; unfold bsm_addstracks', box; try destruct (trans' _ _) as [[[q'?][|]]|]; try split; try apply H1; try apply H2; try apply H3; try lia.
+  now apply Forall_nil.
+Qed.
+
+(* in_code_or_exact_end holds for each POP of P *)
+Lemma P_JMP_spec M1 q1 i:
+  Forall (fun instr : bsm_instr 5 =>
+    match instr with
+      | POP _ k1 k2 =>
+          in_code_or_exact_end k1 q1 (i + 1) /\
+          in_code_or_exact_end k2 q1 (i + 1)
+      | PUSH _ _ => True
+    end)
+  (bsm_addstacks 1 (P M1 q1 (i + 1))).
+Proof.
+  assert (C := c_spec).
+  assert (L := SBTM_HALT_to_HaltBSM.state_map_length_spec M1).
+  unfold P, bsm_addstacks, in_code_or_exact_end.
+  rewrite map_cons, map_app.
+  apply Forall_cons; [| apply Forall_app; split].
+  - cbn.
+    assert (H := state_number_length M1 q1).
+    rewrite length_map, length_app, length_flat_map_PROG_M.
+    lia.
+  - apply Forall_map, Forall_flat_map, Forall_nth.
+    intros.
+    apply PROG_JMP_spec.
+  - repeat apply Forall_cons; unfold bsm_addstracks';  try easy;
+      rewrite !bsm_length; cbn; rewrite length_map, length_app, length_flat_map_PROG_M; simpl; lia.
+Qed.
+
+
+(* P never pushes to STACK*)
+Lemma P_EMPTY_STACK_spec M1 q1 i:
+Forall (fun instr : bsm_instr 5 => 
+  match instr with
+    | POP _ _ _ => True
+    | PUSH STACK _ => STACK <> Fin4
+  end) (bsm_addstacks 1 (P M1 q1 (i + 1))).
+Proof.
+  cbn.
+  rewrite map_app.
+  apply Forall_cons; [easy|].
+  apply Forall_app.
+  split; [|now repeat apply Forall_cons].
+  apply Forall_map, Forall_flat_map, Forall_nth.
+  intros.
+  now (repeat apply Forall_cons); cbn; try destruct (trans' _ _) as [[[??][|]]|].
+Qed.
+
+
+(* If we make a step from (j,v) to (n, t) in FULL_PROG and j lies within the P subprogram, then:
+  1. n lies either within P or is the first code label behind P (first instruction of TRUNC)
+  2. if v[4] empty, then t[4] empty
+*)
+Lemma P_out_code_step_spec M1 q1 i j n t v:
+  in_code j (i + 1, bsm_addstacks 1 (P M1 q1 (i + 1))) ->
+  vec_pos v Fin4 = [] ->
+  sss_step (bsm_sss (n:=5)) (i, FULL_PROG q1 i) (j, v) (n, t) ->
+  @in_code_or_exact_end n M1 q1 (i + 1) /\ vec_pos t Fin4 = [].
+Proof.
+  intros H H0 H1.
+  split. 
+  - assert (H2 := @in_code_step_spec i j n t v 
+    (bsm_addstacks 1 (P M1 q1 (i + 1))) (TRUNC_PROG (i + 1 + (|P M1 q1 (i + 1)|))) INV_TRUNC_PROG).
+    rewrite INV_TRUNC_PROG_length in H2.
+    assert (H3 := P_JMP_spec q1 i).
+    unfold in_code_or_exact_end in H3.
+    now apply (H2 H H3 H1).
+  - assert (H2 := @Step_empty_spec i j n t v 
+    (bsm_addstacks 1 (P M1 q1 (i + 1))) (TRUNC_PROG (i + 1 + (|P M1 q1 (i + 1)|))) INV_TRUNC_PROG Fin4).
+    rewrite INV_TRUNC_PROG_length in H2.
+    now apply (H2 H H0 ((P_EMPTY_STACK_spec q1 i)) H1).
+Qed.
+  
+(* If (j,v) lies withing the P subprogram and if we can go from (j, v) to output (out1, out2),
+    then we can go to (j', v') where j' is behind the code space of the P subprogram.
+    This only holds because of the way FULL_PROG is defined.
+    This is used to get from FULL_PROG to the P subprogram.
+*)
+Lemma P_out_code_spec M1 q1 i j v out1 out2 : 
+  (i, FULL_PROG q1 i) //(j, v) ~~> (out1, out2) ->
+  vec_pos v Fin4 = [] ->
+  in_code (fst (j, v)) (i + 1, bsm_addstacks 1 (P M1 q1 (i + 1))) ->
+    exists j' v',(i + 1, bsm_addstacks 1 (P M1 q1 (i + 1))) // (j, v) ->> (j', v') /\ 
+    code_end (i + 1, bsm_addstacks 1 (P M1 q1 (i + 1))) <= j'.
+Proof.
+  intros [[k H] H1] Q H0.
+  revert out1 out2 v i j H Q H1 H0.
+  induction k as [|k IHk]; intros out1 out2 v i j H Q H1 H0.
+  - apply sss_steps_0_inv in H. injection H. intros H2 H3.
+    cbn in H0. rewrite <- H3 in H1.
+    destruct H1 as [H1 | H1].
+    + cbn in H1. lia.
+    + simpl in H1.
+      rewrite length_map in H0.
+      rewrite !length_app in H1.
+      rewrite (bsm_length 1) in H1.
+      lia.
+  - apply sss_steps_S_inv' in H.
+    destruct H as [[n t] [H' H'']].
+    destruct (P_out_code_step_spec H0 Q H') as [E E1].
+    assert (I : (i + 1, bsm_addstacks 1 (P M1 q1 (i + 1))) <sc (i, FULL_PROG q1 i)) by (unfold FULL_PROG; auto).
+    destruct E as [E | E].
+    + specialize (IHk out1 out2 t i n H'' E1 H1 E).
+      destruct IHk as [j' [v' [[k' IHk1] IHk2]]].
+      exists j', v'.
+      split; [|apply IHk2].
+      exists (S k').
+      apply in_sss_steps_S with (st2 := (n, t)); [apply (sss_step_supcode I H0 H') | apply IHk1].
+    + exists n, t.
+      split.
+      * exists 1.
+          apply sss_steps_1.
+          apply (sss_step_supcode I H0 H').
+      * rewrite E. constructor.
+Qed.
+
+(* ---BSM complete simulation--- *)
+
+(* There is a BSM over 5 stacks that simulates TM M*)
+Lemma BSM_complete_simulation'' n Σ (M : TM Σ n) i :
+  { P |
       (forall q t t', TM.eval M (TM.start M) t q t' ->
-       forall v'', BSM.eval (m + (4)) (i, P) (i, Vector.append v'' ((encode_bsm t))) (i + length P, Vector.append v'' ((encode_bsm t')))) /\
-      (forall t v'', (sss.sss_terminates (bsm_sss (n := (m + (4)))) (i, P) (i, Vector.append v'' ((encode_bsm t)))) -> (exists q' t', TM.eval M (TM.start M) t q' t'))}.
+      BSM.eval 5 (i, P) (i, encode_bsm t) (i + length P, encode_bsm t')) /\
+      (forall t, (exists out, BSM.eval 5 (i, P) (i, encode_bsm t) out) ->
+      (exists q' t', TM.eval M (TM.start M) t q' t'))}.
+Proof.
+  destruct (SBTM_complete_simulation M) as (M1 & q1 & Hf1 & Hb1).
+  exists (FULL_PROG q1 i).
+  split.
+  - clear Hb1.
+    intros q t t' H.
+    rewrite BSM_sss.eval_iff.
+    split; [|right; now constructor].
+    unfold encode_bsm.
+
+    (* SBTM complete encode *)
+    destruct (Hf1 _ _ _ ((complete_encode t)) H (SBTM_facts.almost_eq_tape_refl (complete_encode t))) as [k [q' [t''' [Hf1A [Hf1B Hf1C]]]]]. clear Hf1.
+    apply SBTM_facts.almost_eq_truncate_tape_iff in Hf1C.
+    rewrite <- Hf1C.
+
+    eapply sss_compute_trans; [| eapply sss_compute_trans].
+    + (* INV_TRUNC*)
+      eapply subcode_sss_compute; [| now apply INV_TRUNC_spec].
+      unfold FULL_PROG, INV_TRUNC_PROG.
+      apply sc_spec; [cbn; lia| now replace (i - i) with 0 by lia].
+    + (* P AND ADDSTACKS*)
+      eapply subcode_sss_compute; [| now apply (BSM_addstacks'' [|[]|] (SBTM_HALT_to_HaltBSM.simulation_output' _ _ _ _ _ _ _ Hf1A Hf1B))].
+      eexists (INV_TRUNC_PROG), _.
+      split; [now reflexivity| cbn; lia].
+    + (* TRUNC*)
+      unfold FULL_PROG.
+      rewrite !length_app, bsm_length, INV_TRUNC_PROG_length, !Nat.add_assoc.
+      rewrite <- trunc_order.
+      eapply subcode_sss_compute; [| apply TRUNC_PROG_spec; now destruct t''' as [[??]?]].
+      eexists _, [].
+      split; [now rewrite app_nil_r, app_assoc|].
+      rewrite !length_app, bsm_length. 
+      cbn.
+      lia.
+
+  - intros t H.
+    clear Hf1.
+    apply Hb1.
+    clear Hb1.
+    destruct H as [[out1 out2] H].
+    rewrite BSM_sss.eval_iff in H. 
+    destruct H as [H1 H2].
+    (* REMOVE INVERSE TRUNCATION*)
+    assert (INV : (i, FULL_PROG q1 i) // 
+            (i + 1, vec_app [|[]|](SBTM_HALT_to_HaltBSM.encode_tape (complete_encode t))) ->> (out1, out2)).
+    {
+      destruct H1 as [k H1].
+      apply sss_steps_inv in H1.
+      destruct H1 as [[H1A H1B] | [k' [[st2A st2B] [H1A [H1B H1C]]]]].
+      + injection H1B. clear H1B. intros H1B H1C.
+        assert (H : in_code i ((i, FULL_PROG q1 i))) by (simpl; lia).
+        rewrite <- H1C in H2. 
+        destruct (in_out_code H H2).
+      + apply sss_step_subcode_inv with (ii := PUSH Fin1 false) in H1B. 
+        * apply PUSH_spec in H1B.
+          destruct H1B as [H1B H1D].
+          rewrite H1B, H1D in H1C.
+          exists k'.
+          simpl.
+          rewrite <- truncate_irrel.
+          apply H1C.
+        * eexists [], _.
+          split; [now reflexivity|simpl;lia]. 
+    }
+
+    (* i + 1 is in code of core program P*)
+    assert (IN_CODE : in_code (fst (i + 1,  vec_app [|[]|](SBTM_HALT_to_HaltBSM.encode_tape (complete_encode t)))) (i + 1, bsm_addstacks 1 (P M1 q1 (i + 1)))); [simpl; rewrite (bsm_length 1); lia|].
+    (* REMOVE TRUNCATION *)
+    destruct (P_out_code_spec (conj INV H2) eq_refl IN_CODE) as [j' [v' [[k INV1] INV2]]].
+    unfold code_end, fst, snd in INV2.
+    clear INV H1 IN_CODE H2.
+    (* REMOVE ADD STACKS*)
+    destruct (@BSM_addstacks_bwd' 4 (i + 1) (P M1 q1 (i + 1)) 1 k (i + 1) (SBTM_HALT_to_HaltBSM.encode_tape (complete_encode t)) [|[]|] (j',v') INV1) as [o [v'' [BWD1 BWD2]]]. clear INV1.
+    injection BWD1. intros BWD1A BWD1B. clear BWD1.
+    (* INV SIM*)
+    unfold code_end, fst, snd in INV2.
+    rewrite (bsm_length 1) in INV2.
+    destruct (Nat.le_exists_sub (i + 1 + (| P M1 q1 (i + 1) |)) j' INV2) as [m [LE _]].
+    rewrite Nat.add_comm in LE.
+    rewrite LE in BWD1B.
+    rewrite <- BWD1B in BWD2.
+    rewrite <- Nat.add_assoc in BWD2.
+    apply (SBTM_HALT_to_HaltBSM.inverse_simulation' M1 q1 (i + 1) (complete_encode t) k ((| P M1 q1 (i + 1)|) + m) v'' BWD2).
+    right. simpl. lia.
+Qed.
+
+(* Lift simulation to m + 5 stacks*)
+Lemma BSM_complete_simulation' n Σ (M : TM Σ n) m i :
+  { P |
+      (forall q t t', TM.eval M (TM.start M) t q t' ->
+       forall v'', BSM.eval (m + 5) (i, P) (i, Vector.append v'' ((encode_bsm t))) (i + length P, Vector.append v'' ((encode_bsm t')))) /\
+      (forall t v'', (exists out, BSM.eval (m + 5) (i, P) (i, Vector.append v'' ((encode_bsm t))) out) -> (exists q' t', TM.eval M (TM.start M) t q' t'))}.
+Proof.
+  destruct (BSM_complete_simulation'' M i) as [P [H1 H2]].
+  destruct (BSM_addstacks i P m) as [P' [H3 [H4 H5]]].
+  exists P'.
+  split.
+  - intros q t t' H.
+    apply H4.
+    rewrite <- H3.
+    apply (H1 q t t' H).
+  - intros t v'' [out H].
+    apply H2.
+    apply (H5 (encode_bsm t) v'' i out).
+    apply H.
+Qed.
+
+(* BSM simulation with sss_terminates *)
+Lemma BSM_complete_simulation n Σ (M : TM Σ n) m  i :
+    { P |
+      (forall q t t', TM.eval M (TM.start M) t q t' ->
+       forall v'', BSM.eval (m + 5) (i, P) (i, Vector.append v'' ((encode_bsm t))) (i + length P, Vector.append v'' ((encode_bsm t')))) /\
+      (forall t v'', (sss.sss_terminates (bsm_sss (n := (m + 5))) (i, P) (i, Vector.append v'' ((encode_bsm t)))) ->
+       (exists q' t', TM.eval M (TM.start M) t q' t'))}.
 Proof.
   destruct (@BSM_complete_simulation' n Σ M m i) as (P & H1 & H2).
-  exists P. split.  1: exact H1.
+  exists P. split; [exact H1|].
   intros t v'' ([out1 out2] & H % BSM_sss.eval_iff). eapply H2. eauto.
 Qed.
 
-Local Notation "P // s ->> t" := (sss_compute (@bsm_sss _) P s t).
-
-Lemma pos_right_inj {n m} p q :
-  @pos_right n m p = @pos_right n m q -> p = q.
+(* Check all possible cases of pos 5*)
+Lemma Fin5_cases (P : pos 5 -> Prop) :
+   P Fin0 -> P Fin1 -> P Fin2 -> P Fin3 -> P Fin4 -> forall p, P p.
 Proof.
-  induction n in p, q |- *; cbn in *.
-  - eauto.
-  - intros. eapply IHn, pos_nxt_inj, H.
-Qed.
-
-Lemma vec_pos_const {k} {X x} (p : pos k) : vec_pos (@Vector.const X x k) p = x.
-Proof.
-  induction p; cbn; eauto.
-Qed.
-
-
-Lemma Fin4_cases (P : pos 4 -> Prop) :
-   P Fin0 -> P Fin1 -> P Fin2 -> P Fin3 -> forall p, P p.
-Proof.
-  intros H0 H1 H2 H3.
+  intros H0 H1 H2 H3 H4.
   repeat (intros p; eapply (Fin.caseS' p); clear p; [ eauto | ]).
   intros p. inversion p.
 Qed.
 
 Lemma PREP1_spec k Σ n :
-{ PREP1 : list (bsm_instr ((1 + k) + 4)) | forall v : Vector.t nat k,
-    (0, PREP1) // (0, Vector.append ([] ::: Vector.map (fun n0 : nat => repeat true n0) v) (Vector.const [] 4)) ->>
+{ PREP1 : list (bsm_instr ((1 + k) + 5)) | forall v : Vector.t nat k,
+    (0, PREP1) // (0, Vector.append ([] ::: Vector.map (fun n0 : nat => repeat true n0) v) (Vector.const [] 5)) ->>
                   (length PREP1, Vector.append ([] ::: Vector.map (fun n0 : nat => repeat true n0) v) ((@encode_bsm Σ _ (Vector.const niltape n)))) }.
 Proof.
-  exists (push_exactly (pos_right (1 + k) Fin0) ((@encode_bsm Σ _ (Vector.const niltape n))@[Fin0])
-       ++ push_exactly (pos_right (1 + k) Fin1) ((@encode_bsm Σ _ (Vector.const niltape n))@[Fin1])
-       ++ push_exactly (pos_right (1 + k) Fin2) ((@encode_bsm Σ _ (Vector.const niltape n))@[Fin2])
-       ++ push_exactly (pos_right (1 + k) Fin3) ((@encode_bsm Σ _ (Vector.const niltape n))@[Fin3])).
+  exists (
+      push_exactly (pos_right (1 + k) Fin0) ((@encode_bsm Σ _ (Vector.const niltape n))@[Fin0])
+      ++ push_exactly (pos_right (1 + k) Fin1) ((@encode_bsm Σ _ (Vector.const niltape n))@[Fin1])
+      ++ push_exactly (pos_right (1 + k) Fin2) ((@encode_bsm Σ _ (Vector.const niltape n))@[Fin2])
+      ++ push_exactly (pos_right (1 + k) Fin3) ((@encode_bsm Σ _ (Vector.const niltape n))@[Fin3])
+      ++ push_exactly (pos_right (1 + k) Fin4) ((@encode_bsm Σ _ (Vector.const niltape n))@[Fin4])).
   intros v.
-  eapply subcode_sss_compute_trans. 2: eapply (push_exactly_spec (pos_right (1 + k) Fin0) 0 ((@encode_bsm Σ _ (Vector.const niltape n))@[Fin0])). 1:auto.
+  rewrite <- !vec_app_spec.
+  (* Keeps expressions smaller *)
+  assert (H0 : forall i, @vec_pos (list bool) _ [|[]; []; []; []; []|]  i = []). {
+    do 5 (intros i; apply (Fin.caseS' i); [easy| ]; clear i).
+    now apply (Fin.case0).
+  }
+  eapply subcode_sss_compute_trans; 
+  [| eapply (push_exactly_spec (pos_right (1 + k) Fin0) 0 ((@encode_bsm Σ _ (Vector.const niltape n))@[Fin0]))| ];
+  [now auto |].
+  rewrite vec_change_app_right, vec_pos_app_right, <- vec_pos_spec, H0, vec_pos_spec, encode_bsm_at0.
   eapply subcode_sss_compute_trans. 2: eapply (push_exactly_spec (pos_right (1 + k) Fin1) _ ((@encode_bsm Σ _ (Vector.const niltape n))@[Fin1])). 1:auto.
+  rewrite vec_change_app_right, vec_pos_app_right, <- vec_pos_spec, H0, vec_pos_spec, encode_bsm_at1.
   eapply subcode_sss_compute_trans. 2: eapply (push_exactly_spec (pos_right (1 + k) Fin2) _ ((@encode_bsm Σ _ (Vector.const niltape n))@[Fin2])). 1:auto.
+  rewrite vec_change_app_right, vec_pos_app_right, <- vec_pos_spec, H0, vec_pos_spec, encode_bsm_at2.
   eapply subcode_sss_compute_trans. 2: eapply (push_exactly_spec (pos_right (1 + k) Fin3) _ ((@encode_bsm Σ _ (Vector.const niltape n))@[Fin3])). 1:auto.
-  bsm sss stop. apply f_equal2.
-  1:rewrite !length_app; lia.
-  eapply vec_pos_ext. eapply pos_left_right_rect.
-  - rewrite <- !vec_app_spec. symmetry. rewrite vec_pos_app_left.
-    rewrite !vec_change_neq; auto.
-    now rewrite vec_pos_app_left.
-  - rewrite <- !vec_app_spec. rewrite !vec_pos_app_right.
-    intros p; eapply (Fin.caseS' p); clear p.
-    1:{ repeat (rewrite vec_change_neq; [ | intros ? % pos_right_inj; congruence]).
-        rewrite vec_change_eq; [ | auto]. rewrite vec_pos_app_right.
-        now rewrite vec_pos_const, app_nil_r, vec_pos_spec. }
-    intros p; eapply (Fin.caseS' p); clear p.
-    1:{ rewrite vec_change_neq; [ | intros ? % pos_right_inj % pos_nxt_inj; congruence].
-        rewrite vec_change_neq; [ | intros ? % pos_right_inj % pos_nxt_inj; congruence].
-        rewrite vec_change_eq; [ | auto]. rewrite vec_pos_app_right.
-        rewrite vec_pos_const. rewrite vec_change_neq; [ | intros ? % pos_right_inj; congruence].
-        rewrite vec_pos_app_right. now rewrite vec_pos_const, app_nil_r, vec_pos_spec. }
-    intros p; eapply (Fin.caseS' p); clear p.
-    1:{ rewrite vec_change_neq; [ | intros ? % pos_right_inj % pos_nxt_inj % pos_nxt_inj; congruence].
-        rewrite vec_change_eq; [ | auto]. rewrite vec_pos_app_right.
-        rewrite vec_pos_const. rewrite vec_change_neq; [ | intros ? % pos_right_inj % pos_nxt_inj; congruence].
-        rewrite vec_change_neq; [ | intros ? % pos_right_inj; congruence].
-        rewrite vec_pos_app_right. now rewrite vec_pos_const, app_nil_r, vec_pos_spec. }
-    intros p; eapply (Fin.caseS' p); clear p.
-    1:{ rewrite vec_change_eq; [ | auto]. rewrite vec_pos_app_right.
-        rewrite vec_pos_const. rewrite vec_change_neq; [ | intros ? % pos_right_inj % pos_nxt_inj % pos_nxt_inj; congruence].
-        rewrite vec_change_neq; [ | intros ? % pos_right_inj % pos_nxt_inj; congruence].
-        rewrite vec_change_neq; [ | intros ? % pos_right_inj; congruence].
-        rewrite vec_pos_app_right. now rewrite vec_pos_const, app_nil_r, vec_pos_spec. }
-    apply Fin.case0.
+  rewrite vec_change_app_right, vec_pos_app_right, <- vec_pos_spec.
+  eapply subcode_sss_compute_trans. 2: eapply (push_exactly_spec (pos_right (1 + k) Fin4) _ ((@encode_bsm Σ _ (Vector.const niltape n))@[Fin4])). 1:auto.
+  bsm sss stop. apply f_equal2. 1:rewrite !length_app; lia.
+  rewrite !vec_change_app_right, !app_nil_r, vec_pos_app_right.
+  reflexivity.
 Qed.
 
-Lemma vec_map_spec {X Y n} (v : Vector.t X n) (f : X -> Y) :
-  vec_map f v = Vector.map f v.
+(*
+  encode_bsm always returns the following stacks:
+  0 = []
+  1 = [false]
+  2 = [true]
+  3: no further specification
+  4 = []
+*)
+Lemma encode_bsm_ext Σ n v :
+  @encode_bsm Σ n v = [] ::: [] ::: [true] ::: ((encode_bsm v)@[Fin3]) ::: [] ::: vec_nil.
 Proof.
-  induction v; cbn; congruence.
+  eapply vec_pos_ext. eapply Fin5_cases.
+  - now rewrite vec_pos_spec, encode_bsm_at0.
+  - now rewrite vec_pos_spec, encode_bsm_at1.
+  - now rewrite vec_pos_spec, encode_bsm_at2.
+  - reflexivity.
+  - now rewrite vec_pos_spec, encode_bsm_at4.
 Qed.
 
-Lemma pos_left_inj {n m} p q :
-  @pos_left n m p = @pos_left n m q -> p = q.
-Proof.
-  induction p in q |- *; cbn in *.
-  - eapply (Fin.caseS' q).
-    + reflexivity.
-    + clear q. cbn. congruence.
-  - eapply (Fin.caseS' q).
-    + cbn. congruence.
-    + clear q. cbn. intros. f_equal. eapply IHp.
-      now eapply pos_nxt_inj.
-Qed.
+Opaque encode_bsm.
 
 Lemma PREP2_spec'' k (Σ : finType) (x : pos k) i s b :
-{ PREP2 : list (bsm_instr ((1 + k) + 4)) | length PREP2 = 2 + (length (strpush_common_short s b)) + length ((strpush_succ s b)) /\
-forall v : Vector.t (list bool) k,  forall n, forall t : Vector.t (tape Σ) n, forall m m',
-   v @[x] = repeat true m ->
-    (i, PREP2) // (i,                Vector.append ([] ::: v) ((@encode_bsm Σ _ (encNatTM s b m' ::: t)))) ->>
-                  (i + length PREP2, Vector.append ([] ::: vec_change v x nil) ((@encode_bsm Σ _ (encNatTM s b (m + m') ::: t)))) }.
+{ PREP2 : list (bsm_instr ((1 + k) + 5)) | 
+  length PREP2 = 2 + (length (strpush_common_short s b)) + length ((strpush_succ s b)) /\
+  forall v : Vector.t (list bool) k,  forall n, forall t : Vector.t (tape Σ) n, forall m m',
+    v @[x] = repeat true m ->
+      (i, PREP2) // (i,                Vector.append ([] ::: v) ((@encode_bsm Σ _ (encNatTM s b m' ::: t)))) ->>
+                    (i + length PREP2, Vector.append ([] ::: vec_change v x nil) ((@encode_bsm Σ _ (encNatTM s b (m + m') ::: t)))) }.
 Proof.
-  exists (POP (pos_left 4 (pos_right 1 x)) 0 (i + 2 + (length (strpush_common_short s b)) + length ((strpush_succ s b)))
-       :: pop_many (pos_right (1 + k) Fin2) (length (strpush_common_short s b)) (1 + i)
-       ++ push_exactly (pos_right (1 + k) Fin2) (strpush_succ s b)
-       ++ POP (pos_left 4 Fin0) 0 i :: nil). split.
+  exists (
+        POP (pos_left 5 (pos_right 1 x)) 0 (i + 2 + (length (strpush_common_short s b)) + length ((strpush_succ s b)))
+        :: pop_many (pos_right (1 + k) Fin3) (length (strpush_common_short s b)) (1 + i) 
+        ++ push_exactly (pos_right (1 + k) Fin3) (strpush_succ s b)
+        ++ POP (pos_left 5 Fin0) 0 i
+        :: nil).
+  split.
   { cbn. rewrite !length_app. cbn. rewrite pop_many_length, push_exactly_length. lia. }
   intros v n t m m' Hx.
   induction m in v, m', Hx |- *.
-  - bsm sss POP empty with (pos_left 4 (pos_right 1 x)) 0 (i + 2 + (length (strpush_common_short s b)) + length ((strpush_succ s b))).
-  1: rewrite <- !vec_app_spec, vec_pos_app_left.  1: cbn in *.
-  1: rewrite vec_pos_spec, Hx.  1: reflexivity.
-    bsm sss stop. apply f_equal2.  1: { cbn. rewrite !length_app, pop_many_length, push_exactly_length. cbn. lia. }
-    cbn in Hx. rewrite <- Hx. now rewrite <- vec_pos_spec, vec_change_same.
-  - bsm sss POP one with (pos_left 4 (pos_right 1 x)) 0 (i + 2 + (length (strpush_common_short s b)) + length ((strpush_succ s b))) (repeat true m).
-    1:{ rewrite <- !vec_app_spec, vec_pos_app_left. cbn.
+  - bsm sss POP empty with (pos_left 5 (pos_right 1 x)) 0 (i + 2 + (length (strpush_common_short s b)) + length ((strpush_succ s b))). {
+    rewrite <-!vec_app_spec, vec_pos_app_left. cbn. rewrite vec_pos_spec. easy.
+    }
+    bsm sss stop. apply f_equal2.
+      + cbn. rewrite !length_app, pop_many_length, push_exactly_length. cbn. lia.
+      + cbn in Hx. rewrite <- Hx. now rewrite <- vec_pos_spec, vec_change_same.
+  - bsm sss POP one with (pos_left 5 (pos_right 1 x)) 0 (i + 2 + (length (strpush_common_short s b)) + length ((strpush_succ s b))) (repeat true m).
+     { rewrite <- !vec_app_spec, vec_pos_app_left. cbn.
         rewrite vec_pos_spec, Hx. reflexivity. }
-    eapply subcode_sss_compute_trans. 2: eapply (pop_many_spec (pos_right (1 + k) Fin2) (length (strpush_common_short s b)) (1 + i)). 1:auto.
-    eapply subcode_sss_compute_trans. 2: eapply (push_exactly_spec (pos_right (1 + k) Fin2) _ (strpush_succ s b)).
-    { eexists (POP _ _ _ :: pop_many _ _ _), ([POP _ _ _]). split.
-      1: reflexivity.
-      cbn; rewrite pop_many_length. lia. }
-    bsm sss POP empty with (pos_left 4 Fin0) 0 i. {
-      eexists (POP _ _ _ :: pop_many _ _ _ ++ push_exactly _ _), []. cbn. simpl_list. split. 1: reflexivity.
+    rewrite <- vec_app_spec, vec_change_app_left.
+    replace ([] ::: v) with (vec_app [|[]|] v) by (rewrite vec_app_spec; easy).
+    rewrite vec_change_app_right.
+    eapply subcode_sss_compute_trans. 2: eapply (pop_many_spec (pos_right (1 + k) Fin3) (length (strpush_common_short s b)) (1 + i)). 1:auto.
+    rewrite vec_change_app_right, vec_pos_app_right, encode_bsm_ext.
+    simpl.
+    eapply subcode_sss_compute_trans. 2: eapply (push_exactly_spec (pos_right (1 + k) Fin3) _ (strpush_succ s b)).
+    { eexists (POP _ _ _ :: pop_many _ _ _), ([POP _ _ _]). split; [now reflexivity|].
+      cbn. rewrite pop_many_length. lia. }
+    rewrite vec_change_app_right, vec_pos_app_right.
+    simpl.
+    bsm sss POP empty with (pos_left 5 Fin0) 0 i. {
+      eexists (POP _ _ _ :: pop_many _ _ _ ++ push_exactly _ _), []. cbn. simpl_list. split; [now reflexivity|].
       rewrite pop_many_length, push_exactly_length. lia. }
-    specialize IHm with (m' := (S m')). replace (S m + m') with (m + S m') by lia.
-    match goal with [ |- sss_compute _ _ (_, ?st) _ ] => evar (ev : Vector.t (list bool) ((1 + k) + 4)); enough (st = ev) as ->; subst ev end.
-    1: match goal with [ |- sss_compute _ _ _ (_, ?st) ] => evar (ev : Vector.t (list bool) ((1 + k) + 4)); enough (st = ev) as ->; subst ev end.
-    1: eapply IHm with (v := vec_change v x (repeat true m)).  1: now rewrite <- vec_pos_spec, vec_change_eq.  1: now rewrite vec_change_idem.
-    rewrite <- !vec_app_spec.
-    eapply vec_pos_ext. eapply pos_left_right_rect.
-    + symmetry. rewrite vec_pos_app_left.
-      rewrite vec_change_neq; auto.
-      rewrite vec_change_neq; auto. cbn in p.
-      eapply (Fin.caseS' p); clear p.  1: reflexivity.
-      intros p.
-      destruct (pos_eq_dec p x).
-      * rewrite vec_change_eq. 2: now subst. cbn. subst. now rewrite vec_change_eq.
-      * rewrite vec_change_neq. 2: intros ? % pos_left_inj % pos_nxt_inj; auto.
-        rewrite vec_pos_app_left.  cbn. rewrite vec_change_neq; auto.
-    + intros p. symmetry. rewrite !vec_pos_app_right. symmetry.
-      rewrite !vec_change_idem.
-      revert p.
-      apply Fin4_cases.
-      * repeat (rewrite vec_change_neq; [ | intros ? % pos_right_inj; congruence]).
-          rewrite vec_change_neq; [ | eapply pos_right_left]. rewrite vec_pos_app_right.
-          now rewrite !vec_pos_spec, !encode_bsm_at0.
-      * rewrite vec_change_neq; [ | intros ? % pos_right_inj % pos_nxt_inj; congruence].
-        rewrite vec_change_neq; [ | auto].
-        now rewrite vec_pos_app_right, !vec_pos_spec, !encode_bsm_at1.
-      * rewrite vec_change_eq; auto.
-        rewrite vec_change_eq; auto.
-        rewrite vec_change_neq; auto.
-        rewrite vec_pos_app_right.
-        now rewrite !vec_pos_spec, encode_bsm_succ.
-      * rewrite vec_change_neq; [ | intros ? % pos_right_inj % pos_nxt_inj % pos_nxt_inj; congruence].
-        rewrite vec_change_neq; [ | auto].
-        now rewrite vec_pos_app_right, !vec_pos_spec, !encode_bsm_at3.
+    specialize IHm with (m' := (S m')).
+    match goal with [ |- sss_compute _ _ (_, ?st) _ ] => evar (ev : Vector.t (list bool) ((1 + k) + 5)); enough (st = ev) as ->; subst ev end; [
+    match goal with [ |- sss_compute _ _ _ (_, ?st) ] => evar (ev : Vector.t (list bool) ((1 + k) + 5)); enough (st = ev) as ->; subst ev end|].
+    + eapply IHm with (v := vec_change v x (repeat true m)). now rewrite <- vec_pos_spec, vec_change_eq.
+    + rewrite vec_change_idem; now replace (S (m + m')) with (m + S m') by lia.
+    + rewrite vec_app_spec.
+      f_equal; [now rewrite vec_app_spec| now rewrite <- encode_bsm_succ].
 Qed.
 
 Definition PREP2''_length (Σ : finType) (s b : Σ) := proj1_sig (encode_bsm_zero s b) + length (strpush_zero s b) + 2 + (length (strpush_common_short s b)) + length ((strpush_succ s b)).
 
 Lemma PREP2_spec' k (Σ : finType) (x : pos k) i s b n :
-{ PREP2 : list (bsm_instr ((1 + k) + 4)) | length PREP2 = PREP2''_length s b  /\
-forall v : Vector.t (list bool) k, forall t : Vector.t (tape Σ) n, forall m,
-   v @[x] = repeat true m ->
-    (i, PREP2) // (i,                Vector.append ([] ::: v) ((@encode_bsm Σ _ t))) ->>
-                  (i + length PREP2, Vector.append ([] ::: vec_change v x nil) ((@encode_bsm Σ _ (encNatTM s b m ::: t)))) }.
+{ PREP2 : list (bsm_instr ((1 + k) + 5)) | 
+  length PREP2 = PREP2''_length s b  /\
+  forall v : Vector.t (list bool) k, forall t : Vector.t (tape Σ) n, forall m,
+    v @[x] = repeat true m ->
+      (i, PREP2) // (i,                Vector.append ([] ::: v) ((@encode_bsm Σ _ t))) ->>
+                    (i + length PREP2, Vector.append ([] ::: vec_change v x nil) ((@encode_bsm Σ _ (encNatTM s b m ::: t)))) }.
 Proof.
   unfold PREP2''_length.
   destruct (encode_bsm_zero s b) as [n' Hn'].
   destruct (PREP2_spec'' x (i + n' + length (strpush_zero s b)) s b) as [PREP2 [Hl2 H]].
-  exists (pop_many (pos_right (1 + k) Fin2) n' i
-       ++ push_exactly (pos_right (1 + k) Fin2) (strpush_zero s b)
-       ++ PREP2). split.
+  exists (
+      pop_many (pos_right (1 + k) Fin3) n' i
+       ++ push_exactly (pos_right (1 + k) Fin3) (strpush_zero s b)
+       ++ PREP2).
+  split.
   {  cbn. rewrite !length_app, pop_many_length, push_exactly_length. cbn in Hl2. lia. }
   intros v t m Hm.
-  eapply subcode_sss_compute_trans. 2: eapply (pop_many_spec (pos_right (1 + k) Fin2) n' i). 1:auto.
-  eapply subcode_sss_compute_trans. 2: eapply (push_exactly_spec (pos_right (1 + k) Fin2) _ (strpush_zero s b)).
+  eapply subcode_sss_compute_trans. 2: eapply (pop_many_spec (pos_right (1 + k) Fin3) n' i). 1:auto.
+  rewrite <- vec_app_spec, vec_change_app_right, vec_pos_app_right, encode_bsm_ext.
+  simpl.
+  eapply subcode_sss_compute_trans. 2: eapply (push_exactly_spec (pos_right (1 + k) Fin3) _ (strpush_zero s b)).
   { eexists (pop_many _ _ _), PREP2. split.  1: reflexivity. rewrite pop_many_length. lia. }
+  rewrite vec_change_app_right, vec_pos_app_right.
+  simpl.
   specialize H with (m' := 0) (v := v) (1 := Hm). replace (m + 0) with m in H by lia.
   eapply subcode_sss_compute_trans. 2:{
-  match goal with [ |- sss_compute _ _ (_, ?st) _ ] => evar (ev : Vector.t (list bool) ((1 + k) + 4)); enough (st = ev) as ->; subst ev end.
+  match goal with [ |- sss_compute _ _ (_, ?st) _ ] => evar (ev : Vector.t (list bool) ((1 + k) + 5)); enough (st = ev) as ->; subst ev end.
   1: match goal with [ |- sss_compute _ _ (?st, _) _ ] => evar (ev : nat); enough (st = ev) as ->; subst ev end.
   - eapply H.
   - rewrite push_exactly_length. lia.
-  - eapply vec_pos_ext. eapply pos_left_right_rect.
-    + intros p. rewrite <- !vec_app_spec, !vec_pos_app_left.
-      rewrite vec_change_neq; auto.
-      rewrite vec_change_neq; auto. now rewrite vec_pos_app_left.
-    + rewrite <- !vec_app_spec. eapply Fin4_cases.
-      * rewrite vec_change_neq; [ | intros ? % pos_right_inj; congruence].
-        rewrite vec_change_neq; [ | intros ? % pos_right_inj; congruence].
-        rewrite !vec_pos_app_right.
-        rewrite !vec_pos_spec. now rewrite !encode_bsm_at0.
-      * rewrite vec_change_neq; [ | intros ? % pos_right_inj % pos_nxt_inj; congruence].
-        rewrite vec_change_neq; [ | intros ? % pos_right_inj % pos_nxt_inj; congruence].
-        now rewrite !vec_pos_app_right, !vec_pos_spec, !encode_bsm_at1.
-      * rewrite vec_change_eq; auto.
-        rewrite vec_change_eq; eauto.
-        rewrite !vec_pos_app_right.
-        now rewrite !vec_pos_spec, Hn'.
-      * rewrite vec_change_neq; [ | intros ? % pos_right_inj % pos_nxt_inj % pos_nxt_inj; congruence].
-        rewrite vec_change_neq; [ | intros ? % pos_right_inj % pos_nxt_inj % pos_nxt_inj; congruence].
-        now rewrite !vec_pos_app_right, !vec_pos_spec, !encode_bsm_at3.
+  - rewrite vec_app_spec. f_equal.
+    now rewrite <- Hn', <- encode_bsm_ext.
   }
   { eexists (pop_many _ _ _ ++ push_exactly _ _), []. rewrite app_nil_r. split.  1: now simpl_list. rewrite length_app, pop_many_length, push_exactly_length. lia. }
   bsm sss stop. apply f_equal2; [|reflexivity].
-  rewrite !length_app, pop_many_length, push_exactly_length. lia.
+  now rewrite !length_app, pop_many_length, push_exactly_length, !Nat.add_assoc.
 Qed.
 
-Definition BSM_cast {n} (P : list (bsm_instr n)) {m} (E : n = m) : list (bsm_instr m).
-Proof. subst m. exact P. Defined.
-
-Lemma BSM_cast_length {n} (P : list (bsm_instr n)) {m} (E : n = m) :
-  length (BSM_cast P E) = length P.
-Proof.
-  destruct E. cbn. reflexivity.
-Qed.
-
-Lemma BSM_cast_spec {n m} i (P : list (bsm_instr n)) (E : n = m) j v k w :
-   sss.sss_compute (@bsm_sss _) (i, P) (j, v) (k, w) <-> sss.sss_compute (@bsm_sss _) (i, BSM_cast P E) (j, Vector.cast v E) (k, Vector.cast w E).
-Proof.
-  destruct E. cbn. now rewrite !cast_eq_refl.
-Qed.
-
-Fixpoint PREP2' (Σ : finType) (s b : Σ) k'' (k' : nat)  (i : nat) (n : nat) : list (bsm_instr ((1 + (k' + k'') + 4))).
+Fixpoint PREP2' (Σ : finType) (s b : Σ) k'' (k' : nat)  (i : nat) (n : nat) : list (bsm_instr ((1 + (k' + k'') + 5))).
 Proof.
   destruct k'.
   - exact List.nil.
@@ -723,8 +1637,8 @@ Qed.
 Notation "v1 +++ v2" := (Vector.append v1 v2) (at level 60).
 
 Lemma vec_list_encode_bsm Σ n1 n2 v1 v2 :
-vec_list v1 = vec_list v2 ->
- vec_list (@encode_bsm Σ n1 v1) = vec_list (@encode_bsm Σ n2 v2).
+  vec_list v1 = vec_list v2 ->
+  vec_list (@encode_bsm Σ n1 v1) = vec_list (@encode_bsm Σ n2 v2).
 Proof.
   intros H.
   assert (n1 = n2).  1: eapply (f_equal (@length _)) in H.  1: rewrite !vec_list_length in H.  1: assumption.
@@ -733,8 +1647,8 @@ Qed.
 
 Lemma PREP2_spec_strong (Σ : finType) i s b k' k'' v (v' : Vector.t nat k'') n (t : Vector.t (tape Σ) n) :
     (i, @PREP2' Σ s b k'' k'  i n) //
-        (i,                                            ([] ::: Vector.map (fun n => repeat true n) v +++ Vector.const [] k'') +++  (@encode_bsm Σ _ (Vector.map (encNatTM s b) v' +++ t))) ->>
-        (i + length(@PREP2' Σ s b k'' k' i n), ([] ::: Vector.const [] (k' + k'')  +++  (@encode_bsm Σ _ (Vector.map (encNatTM s b) (v +++ v') +++ t)))).
+    (i,                                    ([] ::: Vector.map (fun n => repeat true n) v +++ Vector.const [] k'') +++  (@encode_bsm Σ _ (Vector.map (encNatTM s b) v' +++ t))) ->>
+    (i + length(@PREP2' Σ s b k'' k' i n), ([] ::: Vector.const [] (k' + k'')  +++  (@encode_bsm Σ _ (Vector.map (encNatTM s b) (v +++ v') +++ t)))).
 Proof.
   induction k' in k'', v, v', i |- *.
   - cbn. bsm sss stop. f_equal.  1: lia. f_equal. revert v. apply (Vector.case0). reflexivity.
@@ -750,11 +1664,11 @@ Proof.
     erewrite nth_error_vec_list.
     all:eapply (nth_error_nth' _ 0); rewrite vec_list_length; lia. }
     pose proof (@vec_list_vec_map nat (list bool)) as Heq. specialize (Heq) with (n := (S (k' + k''))).
-    match goal with [ |- sss_compute _ _ (_, ?st) _ ] => evar (ev : vec (list bool) (S (S (k' + k'' + 4)))); enough (st = ev) as ->; subst ev end.
-    1: match goal with [ |- sss_compute _ _ _ (_, ?st) ] => evar (ev : vec (list bool) (S (S (k' + k'' + 4)))); enough (st = ev) as ->; subst ev end.
+    match goal with [ |- sss_compute _ _ (_, ?st) _ ] => evar (ev : vec (list bool) (S (S (k' + k'' + 5)))); enough (st = ev) as ->; subst ev end.
+    1: match goal with [ |- sss_compute _ _ _ (_, ?st) ] => evar (ev : vec (list bool) (S (S (k' + k'' + 5)))); enough (st = ev) as ->; subst ev end.
     1: match goal with [ |- sss_compute _ _ _ (?st, _) ] => evar (ev : nat); enough (st = ev) as ->; subst ev end.
     1: cbn - [minus mult] in HlP.  1: rewrite <- HlP.
-    1: eapply subcode_sss_compute with (P := (i + |PREPIT|, _)). { exists PREPIT, []. split. 2:reflexivity. now simpl_list. }
+    1: eapply subcode_sss_compute with (P := (i + (|PREPIT|), _)). { exists PREPIT, []. split. 2:reflexivity. now simpl_list. }
     1: specialize IHk' with (v := vl) (v' := y ::: v') (k'' := S k'').  1: apply BSM_cast_spec.
     1: eapply IHk'.
     + rewrite !length_app, BSM_cast_length, !PREP2'_length.
@@ -763,7 +1677,8 @@ Proof.
       rewrite <- !vec_map_spec, <- !vec_app_spec. cbn [vec_list]. rewrite !vec_list_cast, !vec_list_vec_app, !vec_list_const.
       rewrite app_comm_cons. f_equal.
       1: now replace  (k' + S k'') with (S (k' + k'')) by lia. f_equal. subst v.
-      rewrite !vec_app_spec. setoid_rewrite vec_map_spec.
+      rewrite !vec_app_spec.
+      rewrite vec_map_spec.
       rewrite !Vector_map_app.
       pose proof (@Vector_map_app) as Vm. specialize Vm with (k1 := S k') (k2 := k''). cbn in Vm. rewrite Vm. clear Vm.
       eapply vec_list_inj, vec_list_encode_bsm.
@@ -776,32 +1691,37 @@ Proof.
       rewrite !vec_list_cast, vec_list_vec_app. cbn. simpl_list. reflexivity.
     + eapply vec_list_inj. rewrite <- !vec_map_spec, <- !vec_app_spec. cbn [vec_list].
       rewrite !vec_list_cast.
-       pose proof (@vec_list_vec_app (list bool) (S (k' + k'')) 4). cbn [plus] in H. rewrite !H. clear H.
-       pose proof (@vec_list_vec_app (list bool) (S (k' + S k'')) 4). cbn [plus] in H. rewrite !H. clear H.
-       cbn [vec_list app]. f_equal. rewrite !vec_list_vec_app.
-       cbn [Vector.map]. rewrite vec_app_cons. f_equal. 2:{ f_equal. f_equal. f_equal.
-       subst v. f_equal. rewrite <- vec_pos_spec. eapply nth_error_vec_list.
-       rewrite vec_list_cast, <- vec_app_spec, vec_list_vec_app, nth_error_app2; rewrite !vec_list_length, ?Nat.sub_diag; try lia.
-       reflexivity. }
-       rewrite vec_list_vec_change.
-       pose proof (@vec_list_vec_app (list bool) (S k') k''). cbn [plus] in H. rewrite !H. clear H.
-       setoid_rewrite <- vec_map_spec.
-       rewrite !vec_list_vec_map, !vec_list_const.
-       rewrite update_app_left. 2: rewrite Fin.to_nat_of_nat; cbn; rewrite length_map, vec_list_length; lia.
-       subst v. rewrite vec_list_cast. rewrite <- vec_app_spec. rewrite vec_list_vec_app. cbn [vec_list]. rewrite Fin.to_nat_of_nat. cbn.
-       rewrite map_app, update_app_right.  2: rewrite length_map, vec_list_length; lia.
-       rewrite length_map, vec_list_length, Nat.sub_diag. cbn. now simpl_list.
+      pose proof (@vec_list_vec_app (list bool) (S (k' + k'')) 5). cbn [plus] in H. rewrite !H. clear H.
+      pose proof (@vec_list_vec_app (list bool) (S (k' + S k'')) 5). cbn [plus] in H. rewrite !H. clear H.
+      cbn [vec_list app].
+      f_equal.
+      rewrite !vec_list_vec_app.
+      cbn [Vector.map]. rewrite vec_app_cons. f_equal. 2:{
+      cbn.
+      rewrite Hv, <- vec_pos_spec.
+      repeat f_equal.
+      eapply nth_error_vec_list.
+      rewrite vec_list_cast, <- vec_app_spec, vec_list_vec_app, nth_error_app2; rewrite !vec_list_length, ?Nat.sub_diag; try lia.
+      reflexivity. }
+      rewrite vec_list_vec_change.
+      pose proof (@vec_list_vec_app (list bool) (S k') k''). cbn [plus] in H. rewrite !H. clear H.
+      setoid_rewrite <- vec_map_spec.
+      rewrite !vec_list_vec_map, !vec_list_const.
+      rewrite update_app_left. 2: rewrite Fin.to_nat_of_nat; cbn; rewrite length_map, vec_list_length; lia.
+      subst v. rewrite vec_list_cast. rewrite <- vec_app_spec. rewrite vec_list_vec_app. cbn [vec_list]. rewrite Fin.to_nat_of_nat. cbn.
+      rewrite map_app, update_app_right.  2: rewrite length_map, vec_list_length; lia.
+      rewrite length_map, vec_list_length, Nat.sub_diag. cbn. now simpl_list.
 Qed.
 
 Lemma PREP2_spec k (Σ : finType) i s b  n :
   { PREP2 | forall v (t : Vector.t (tape Σ) n),
     (i, PREP2) //
-        (i,                               ([] ::: Vector.map (fun n => repeat true n) v) +++  (@encode_bsm Σ _ t)) ->>
-        (i + length PREP2, ([] ::: Vector.const [] k                      +++  (@encode_bsm Σ _ (Vector.map (encNatTM s b) v +++ t)))) }.
+    (i,                ([] ::: Vector.map (fun n => repeat true n) v) +++  (@encode_bsm Σ _ t)) ->>
+    (i + length PREP2, ([] ::: Vector.const [] k                      +++  (@encode_bsm Σ _ (Vector.map (encNatTM s b) v +++ t)))) }.
 Proof.
   unshelve eexists (BSM_cast (@PREP2' Σ s b 0 k  i n) _).  1: abstract lia. intros v t.
-  match goal with [ |- sss_compute _ _ (_, ?st) _ ] => evar (ev : vec (list bool) (S k + 4)); enough (st = ev) as ->; subst ev end.
-  1: match goal with [ |- sss_compute _ _ _ (_, ?st) ] => evar (ev : vec (list bool) (S k + 4)); enough (st = ev) as ->; subst ev end.
+  match goal with [ |- sss_compute _ _ (_, ?st) _ ] => evar (ev : vec (list bool) (S k + 5)); enough (st = ev) as ->; subst ev end.
+  1: match goal with [ |- sss_compute _ _ _ (_, ?st) ] => evar (ev : vec (list bool) (S k + 5)); enough (st = ev) as ->; subst ev end.
   1: rewrite <- BSM_cast_spec.
   1: rewrite BSM_cast_length.  1: eapply PREP2_spec_strong.
     - eapply vec_list_inj.
@@ -823,41 +1743,26 @@ Lemma PREP3_spec k n Σ i :
   }.
 Proof.
   edestruct (@encode_bsm_nil Σ n) as ([str n'] & H).
-  exists (pop_many (pos_right k Fin2) n' i
-      ++ push_exactly (pos_right k Fin2) str).
+  exists (pop_many (pos_right k Fin3) n' i
+      ++ push_exactly (pos_right k Fin3) str).
   intros v t.
-  eapply subcode_sss_compute_trans with (P := (i, pop_many (pos_right k Fin2) n' i)).  1: auto.
+  eapply subcode_sss_compute_trans with (P := (i, pop_many (pos_right k Fin3) n' i)).  1: auto.
   1: eapply pop_many_spec.
-  eapply subcode_sss_compute_trans with (P := (n' + i, push_exactly (pos_right k Fin2) str)).
-  { exists (pop_many (pos_right k Fin2) n' i), []. split.  1: now rewrite app_nil_r. rewrite pop_many_length; lia. }
+  rewrite <- vec_app_spec, vec_change_app_right.
+  eapply subcode_sss_compute_trans with (P := (n' + i, push_exactly (pos_right k Fin3) str)).
+  { exists (pop_many (pos_right k Fin3) n' i), []. split.  1: now rewrite app_nil_r. rewrite pop_many_length; lia. }
   1: eapply push_exactly_spec. bsm sss stop.
-  f_equal.  1: rewrite length_app, pop_many_length, push_exactly_length; lia.
-  rewrite !vec_change_idem.
-  rewrite vec_change_eq; auto.
-  rewrite <- !vec_app_spec.
-  rewrite vec_pos_app_right.
-  eapply vec_pos_ext.  eapply pos_left_right_rect.
-  - intros p. rewrite vec_pos_app_left.
-    rewrite vec_change_neq; auto. now  rewrite vec_pos_app_left.
-  - eapply Fin4_cases.
-    + rewrite !vec_pos_app_right.
-      rewrite vec_change_neq; [ | intros ? % pos_right_inj; congruence].
-      rewrite vec_pos_app_right. now rewrite !vec_pos_spec, !encode_bsm_at0.
-    + rewrite !vec_pos_app_right.
-      rewrite vec_change_neq; [ | intros ? % pos_right_inj % pos_nxt_inj; congruence].
-      rewrite vec_pos_app_right. now rewrite !vec_pos_spec, !encode_bsm_at1.
-    + rewrite !vec_pos_app_right.
-      rewrite vec_change_eq; auto.
-      now rewrite !vec_pos_spec, H.
-    + rewrite !vec_pos_app_right.
-      rewrite vec_change_neq; [ | intros ? % pos_right_inj % pos_nxt_inj % pos_nxt_inj; congruence].
-      rewrite vec_pos_app_right. now rewrite !vec_pos_spec, !encode_bsm_at3.
+  f_equal.  1: rewrite length_app, pop_many_length, push_exactly_length, push_exactly_length; lia.
+  rewrite vec_change_app_right, vec_app_spec, !vec_pos_app_right, vec_change_idem, encode_bsm_ext.
+  simpl.
+  now rewrite <- H, encode_bsm_ext.
 Qed.
+
 
 Lemma PREP_spec k n Σ s b :
   { PREP | forall v : Vector.t nat k,
-    (0, PREP) // (0, Vector.append ([] ::: Vector.map (fun n0 : nat => repeat true n0) v) (Vector.const [] 4)) ->>
-                                           (length PREP, Vector.append (Vector.const [] (1 + k)) ((@encode_bsm Σ _ (Vector.append (niltape ::: Vector.map (encNatTM s b) v)
+    (0, PREP) // (0, Vector.append ([] ::: Vector.map (fun n0 : nat => repeat true n0) v) (Vector.const [] 5)) ->>
+                 (length PREP, Vector.append (Vector.const [] (1 + k)) ((@encode_bsm Σ _ (Vector.append (niltape ::: Vector.map (encNatTM s b) v)
                                            (Vector.const niltape n)))))
   }.
 Proof.
@@ -887,41 +1792,59 @@ Lemma vec'_pos_app_right {X : Type} (n m : nat) (v : vec X n) (w : vec X m) (i :
   vec_pos (v +++ w) (pos_right n i) = vec_pos w i.
 Proof. rewrite <- !vec_app_spec. apply vec_pos_app_right. Qed.
 
+Lemma flat_map_encode_symbol_inj v1 v2 :
+  flat_map encode_symbol v1 = flat_map encode_symbol v2 -> v1 = v2.
+Proof.
+  revert v2.
+  induction v1 as [| a l1]; intros v2 H; destruct v2 as [| b l2]; [easy| inversion H | inversion H|]; destruct a,b; [|inversion H|inversion H|];
+  f_equal; apply IHl1; cbn in H; injection H; easy.
+Qed.
+  
+Transparent encoding_func.
+
 Lemma POSTP_spec' k n (Σ : finType) s b i :
   { POSTP | forall v : Vector.t _ k, forall t : Vector.t (tape Σ) (k + n), forall m m', exists out,
-   (i, POSTP) // (i, Vector.append (repeat true m' ## v) ([] ::: [false] ::: skipn (length (strpush_common s b)) ((encode_bsm (encNatTM s b m ## t))@[Fin2]) ::: [] ::: vec_nil)) ->>
+   (i, POSTP) // (i, Vector.append (repeat true m' ## v) ([] ::: [] ::: [true] ::: skipn (length (strpush_common s b)) ((encode_bsm (encNatTM s b m ## t))@[Fin3]) ::: [] ::: vec_nil)) ->>
                  (i + length POSTP, Vector.append (repeat true (m + m') ## v) (out ))
   }.
 Proof.
-  pose (THESYM := encode_sym
-  (projT1
-     (projT2
-        (FinTypes.finite_n
-           (finType_CS
-              (boundary +
-               sigList (EncodeTapes.sigTape Σ)))))
-     (inr (sigList_X (EncodeTapes.UnmarkedSymbol s))))).
-  exists (pop_exactly (pos_right (1 + k) Fin2) (pos_right (1 + k) Fin0) (i + 4 + 2 * length THESYM) THESYM i
-      ++  PUSH (pos_left 4 Fin0) true
-      ::  pop_many (pos_right (1 + k) Fin2) 2 (i + 1 + 2 * length THESYM)
+  pose (THESYM := flat_map encode_symbol (encoding_func ((inr (sigList_X (EncodeTapes.UnmarkedSymbol s)))))).
+  exists (
+      pop_exactly (pos_right (1 + k) Fin3) (pos_right (1 + k) Fin4) (i + 6 + 2 * length THESYM) THESYM i
+      ++  PUSH (pos_left 5 Fin0) true
+      ::  pop_many (pos_right (1 + k) Fin3) 4 (i + 1 + 2 * length THESYM)
       ++  POP (pos_right (1 + k) Fin0) i i :: nil).
+
+  assert (ENC : forall v, | flat_map encode_symbol v | = 2 * (|v|)). {
+    induction v as [| a l]; [cbn; lia|].
+    cbn.
+    cbn in IHl. rewrite IHl.
+    unfold "*".
+    rewrite !Nat.add_0_r, <- Nat.add_succ_r, <- Nat.add_succ_l.
+    reflexivity.
+  }
   intros.
   induction m in i, m' |- *.
   - pose proof (encode_bsm_zero s b) as [n' Hn'].
     rewrite Hn'. unfold strpush_zero. rewrite <- !app_assoc.
     rewrite skipn_app'; [ | reflexivity].
-    edestruct (@pop_exactly_spec2 (1 + k + 4) (pos_right (1 + k) Fin2) (pos_right (1 + k) Fin0) (i + 4 + 2 * length THESYM)) as [x' Hpop].
-    1:{ intros ? % pos_right_inj; congruence. }
+    edestruct (@pop_exactly_spec2 (1 + k + 5) (pos_right (1 + k) Fin3) (pos_right (1 + k) Fin4) (i + 6 + 2 * length THESYM)) as [x' Hpop].
+    1:{ intros ? % pos_right_inj. discriminate. }
     3:{ eexists. eapply subcode_sss_compute_trans. 2: eapply Hpop.  1: auto.  1: eexists [], _.  1: cbn.  1: split. 2: lia.  1: reflexivity.
         bsm sss stop. apply f_equal2. 1: rewrite !length_app, pop_exactly_length.  1: cbn - [mult].  1: lia.
         apply vec'_change_app_right. }
     2:{ apply vec'_pos_app_right. }
        rewrite vec'_pos_app_right. cbn.
     intros (l' & Hneq).
-     unfold THESYM in Hneq. eapply utils_list.list_app_inj in Hneq as [].
-     2: now rewrite !length_encode_sym. eapply encode_sym_inj in H.
-     clear - H. destruct FinTypes.finite_n as [? [f H']]; cbn in *.
-     destruct H' as [g [_ H2]]. eapply (f_equal g) in H. now rewrite !H2 in H.
+    unfold THESYM in Hneq. eapply utils_list.list_app_inj in Hneq as [].
+    2: 
+    unfold encoding_func; 
+    repeat rewrite ENC; now rewrite !length_encode_sym.
+    unfold encoding_func, encoding_func' in H.
+    eapply flat_map_encode_symbol_inj in H.
+    eapply encode_sym_inj in H.
+    clear - H. destruct FinTypes.finite_n as [? [f H']]; cbn in *.
+    destruct H' as [g [_ H2]]. eapply (f_equal g) in H. now rewrite !H2 in H.
   - edestruct IHm as [out IH]. eexists.
     rewrite encode_bsm_succ. unfold strpush_succ. fold THESYM. rewrite <- !app_assoc.
     rewrite skipn_app' by reflexivity.
@@ -930,51 +1853,36 @@ Proof.
     1: { cbn. rewrite vec'_pos_app_right. cbn. 1: reflexivity. }
     1: { apply vec'_pos_app_right. }
     rewrite <- !vec_app_spec. rewrite vec_app_cons. cbn [vec_change pos_S_inv]. rewrite vec_change_app_right. cbn [vec_change pos_S_inv].
-    bsm sss PUSH with  (pos_left 4 Fin0) true.  1: eexists (pop_exactly (pos_right (1 + k) pos2) (pos_right (1 + k) pos0)
-    (i + 4 + 2 * (| THESYM |)) THESYM i), _.  1: { cbn. split. 1: reflexivity. rewrite pop_exactly_length. lia. }
-
-    
+    bsm sss PUSH with  (pos_left 5 Fin0) true.  1: eexists (pop_exactly (pos_right (1 + k) pos3) (pos_right (1 + k) pos4)
+    (i + 6 + 2 * (| THESYM |)) THESYM i), _.  1: { cbn. split. 1: reflexivity. rewrite pop_exactly_length. lia. }
     rewrite <- vec_app_cons. rewrite vec_change_app_left. cbn [vec_change pos_S_inv]. rewrite vec_pos_app_left. cbn [vec_pos pos_S_inv].
-    eapply subcode_sss_compute_trans. 2: eapply (@pop_many_spec (1 + k + 4) (pos_right (1 + k) Fin2) 2).
-    { eexists (pop_exactly (pos_right (1 + k) Fin2) (pos_right (1 + k) Fin0) (i + 4 + 2 * length THESYM) THESYM i
-    ++  PUSH (pos_left 4 Fin0) true :: nil), (POP (pos_right (1 + k) Fin0) i i :: nil). split.  1: simpl_list.  1: cbn - [mult].  1: repeat f_equal. 1-4: cbn; lia.
+    eapply subcode_sss_compute_trans. 2: eapply (@pop_many_spec (1 + k + 5) (pos_right (1 + k) Fin3) 4).
+    { eexists (pop_exactly (pos_right (1 + k) Fin3) (pos_right (1 + k) Fin4) (i + 6 + 2 * length THESYM) THESYM i
+    ++  PUSH (pos_left 5 Fin0) true :: nil), (POP (pos_right (1 + k) Fin0) i i :: nil). split.  1: simpl_list.  1: cbn - [mult].  1: repeat f_equal. 1-8: cbn; lia.
     rewrite length_app, pop_exactly_length. cbn. lia. }
     rewrite vec_change_app_right. cbn [vec_change pos_S_inv]. rewrite vec_pos_app_right.
     cbn [vec_pos pos_S_inv]. rewrite skipn_plus.
     bsm sss POP empty with (pos_right (1 + k) Fin0) i i.  1: eexists (_ ++ _ :: _), [].  1: split.  1: rewrite app_nil_r.  1: simpl_list.  1: reflexivity.  1: rewrite length_app, pop_exactly_length.
     1: cbn.  1: lia.  1: now rewrite vec_pos_app_right.
-    
-
-    match goal with [ |- sss_compute _ _ (_, ?st) _ ] => evar (ev : Vector.t (list bool) ((1 + k) + 4)); enough (st = ev) as ->; subst ev end.
-    1: match goal with [ |- sss_compute _ _ (_, _) (_, ?st) ] => evar (ev : Vector.t (list bool) ((1 + k) + 4)); enough (st = ev) as ->; subst ev end.
+    match goal with [ |- sss_compute _ _ (_, ?st) _ ] => evar (ev : Vector.t (list bool) ((1 + k) + 5)); enough (st = ev) as ->; subst ev end.
+    1: match goal with [ |- sss_compute _ _ (_, _) (_, ?st) ] => evar (ev : Vector.t (list bool) ((1 + k) + 5)); enough (st = ev) as ->; subst ev end.
     1: eapply IH.  1: instantiate (1 := S m').  1: replace (m + S m') with (S (m + m')).  1: cbn [repeat plus].  1: rewrite vec_app_cons.
     1: now rewrite vec_app_spec.  1: lia.
     cbn [repeat]. rewrite vec_app_spec.
-    assert (2 + (| strpush_common_short s b |) = | strpush_common s b |) as ->.
+    assert (4 + (| strpush_common_short s b |) = | strpush_common s b |).
     { unfold strpush_common. rewrite length_app. cbn. lia. }
-    reflexivity.
-Qed.
-
-Lemma encode_bsm_ext Σ n v :
-  @encode_bsm Σ n v = [] ::: [false] ::: (encode_bsm v @[Fin2]) ::: [] ::: vec_nil.
-Proof.
-  eapply vec_pos_ext. eapply Fin4_cases.
-  - now rewrite vec_pos_spec, encode_bsm_at0.
-  - now rewrite vec_pos_spec, encode_bsm_at1.
-  - reflexivity.
-  - now rewrite vec_pos_spec, encode_bsm_at3.
+    now rewrite <- H.
 Qed.
 
 Lemma POSTP_spec k n (Σ : finType) s b i :
   { POSTP | forall v : Vector.t _ k, forall t : Vector.t (tape Σ) (k + n), forall m, exists out,
    (i, POSTP) // (i, Vector.append ([] ## v) ((encode_bsm (encNatTM s b m ## t)))) ->>
-                                            (i + length POSTP, Vector.append (repeat true m ## v) (out ))
+                 (i + length POSTP, Vector.append (repeat true m ## v) (out ))
   }.
 Proof.
   destruct (@POSTP_spec' k n Σ s b (i + (length (strpush_common s b)))) as [POSTP HPOST].
   specialize HPOST with (m' := 0).
-  exists (pop_many (pos_right (1 + k) Fin2) (length (strpush_common s b)) i
-      ++  POSTP).
+  exists (pop_many (pos_right (1 + k) Fin3) (length (strpush_common s b)) i ++ POSTP).
   intros v t m. specialize HPOST with (m := m).
   edestruct (HPOST v) as (out & HPOST').
   exists out.
@@ -986,7 +1894,7 @@ Proof.
   rewrite vec_app_spec. cbn [Vector.append] in *.
   rewrite vec_app_cons.
   rewrite Nat.add_0_r in HPOST'. rewrite vec_app_spec. cbn [repeat] in HPOST'.
-  replace (|strpush_common s b| + i) with (i + |strpush_common s b|) by lia.
+  replace ((|strpush_common s b|) + i) with (i + (|strpush_common s b|)) by lia.
   eapply subcode_sss_compute_trans.
   2: apply HPOST'.  1: eexists _, [].  1: split.  1: now rewrite app_nil_r.  1: rewrite pop_many_length.  1: lia.
   bsm sss stop. f_equal. rewrite length_app, pop_many_length. cbn. lia.
